update

theory/Sound_Semantics.thy
@@ -88,7 +88,7 @@ inductive static_eval_stack :: "abstract_value_env \<times> abstract_value_env \
   "
 
 
-inductive accept_state :: "abstract_value_env \<times> abstract_value_env \<Rightarrow> state \<Rightarrow> bool" (infix "\<Turnstile>\<^sub>\<sigma>" 55)  where
+inductive static_eval_state :: "abstract_value_env \<times> abstract_value_env \<Rightarrow> state \<Rightarrow> bool" (infix "\<Turnstile>\<^sub>\<sigma>" 55)  where
   Any: "
     \<lbrakk>
       (\<V>, \<C>) \<Turnstile>\<^sub>e e;
@@ -105,17 +105,17 @@ inductive static_eval_pool :: "abstract_value_env \<times> abstract_value_env \<
     (\<V>, \<C>) \<Turnstile>\<^sub>\<E> \<E>
   "
 
-lemma accept_state_to_exp_result: "
+lemma static_eval_state_to_exp_result: "
   (\<V>, \<C>) \<Turnstile>\<^sub>\<sigma> \<langle>RESULT x;\<rho>;\<langle>x\<^sub>\<kappa>,e\<^sub>\<kappa>,\<rho>\<^sub>\<kappa>\<rangle> # \<kappa>\<rangle> \<Longrightarrow> (\<V>, \<C>) \<Turnstile>\<^sub>e e\<^sub>\<kappa>
 "
 proof -
  assume "(\<V>, \<C>) \<Turnstile>\<^sub>\<sigma> \<langle>RESULT x;\<rho>;\<langle>x\<^sub>\<kappa>,e\<^sub>\<kappa>,\<rho>\<^sub>\<kappa>\<rangle> # \<kappa>\<rangle>" then
- have "(\<V>, \<C>) \<Turnstile>\<^sub>\<kappa> \<V> x \<Rrightarrow> \<langle>x\<^sub>\<kappa>,e\<^sub>\<kappa>,\<rho>\<^sub>\<kappa>\<rangle> # \<kappa>" by (simp add: accept_state.simps) then
+ have "(\<V>, \<C>) \<Turnstile>\<^sub>\<kappa> \<V> x \<Rrightarrow> \<langle>x\<^sub>\<kappa>,e\<^sub>\<kappa>,\<rho>\<^sub>\<kappa>\<rangle> # \<kappa>" by (simp add: static_eval_state.simps) then
  show "(\<V>, \<C>) \<Turnstile>\<^sub>e e\<^sub>\<kappa>" by (rule static_eval_stack.cases; auto)
 qed
 
 
-lemma accept_state_to_exp_let_case_left: "
+lemma static_eval_state_to_exp_let_case_left: "
   (\<V>, \<C>) \<Turnstile>\<^sub>\<sigma> \<langle>LET x = CASE x\<^sub>s LEFT x\<^sub>l |> e\<^sub>l RIGHT x\<^sub>r |> e\<^sub>r in e; \<rho>; \<kappa>\<rangle> \<Longrightarrow> 
   \<rho> x\<^sub>s = Some \<lbrace>prim.Left x\<^sub>l', \<rho>\<^sub>l\<rbrace> \<Longrightarrow> 
   (\<V>, \<C>) \<Turnstile>\<^sub>e e\<^sub>l
@@ -125,7 +125,7 @@ proof -
   assume "(\<V>, \<C>) \<Turnstile>\<^sub>\<sigma> \<langle>LET x = CASE x\<^sub>s LEFT x\<^sub>l |> e\<^sub>l RIGHT x\<^sub>r |> e\<^sub>r in e; \<rho>; \<kappa>\<rangle>" then
   have "(\<V>, \<C>) \<Turnstile>\<^sub>e LET x = CASE x\<^sub>s LEFT x\<^sub>l |> e\<^sub>l RIGHT x\<^sub>r |> e\<^sub>r in e"  
   and "(\<V>, \<C>) \<Turnstile>\<^sub>\<rho> \<rho>"
-  by (simp add: accept_state.simps)+ then
+  by (simp add: static_eval_state.simps)+ then
   have "\<forall>x \<omega>. \<rho> x = Some \<omega> \<longrightarrow> {|\<omega>|} \<subseteq> \<V> x" by (simp add: static_eval_env.simps)
   with `\<rho> x\<^sub>s = Some \<lbrace>prim.Left x\<^sub>l', \<rho>\<^sub>l\<rbrace>`
   have "^prim.Left x\<^sub>l' \<in> \<V> x\<^sub>s" by fastforce
@@ -141,7 +141,7 @@ proof -
 qed
 
 
-lemma accept_state_to_exp_let_case_right: "
+lemma static_eval_state_to_exp_let_case_right: "
   (\<V>, \<C>) \<Turnstile>\<^sub>\<sigma> \<langle>LET x = CASE x\<^sub>s LEFT x\<^sub>l |> e\<^sub>l RIGHT x\<^sub>r |> e\<^sub>r in e; \<rho>; \<kappa>\<rangle> \<Longrightarrow> 
   \<rho> x\<^sub>s = Some \<lbrace>prim.Right x\<^sub>r', \<rho>\<^sub>r\<rbrace> \<Longrightarrow> 
   (\<V>, \<C>) \<Turnstile>\<^sub>e e\<^sub>r
@@ -151,7 +151,7 @@ proof -
   assume "(\<V>, \<C>) \<Turnstile>\<^sub>\<sigma> \<langle>LET x = CASE x\<^sub>s LEFT x\<^sub>l |> e\<^sub>l RIGHT x\<^sub>r |> e\<^sub>r in e; \<rho>; \<kappa>\<rangle>" then
   have "(\<V>, \<C>) \<Turnstile>\<^sub>e LET x = CASE x\<^sub>s LEFT x\<^sub>l |> e\<^sub>l RIGHT x\<^sub>r |> e\<^sub>r in e"  
   and "(\<V>, \<C>) \<Turnstile>\<^sub>\<rho> \<rho>" 
-    by (simp add: accept_state.simps)+ then
+    by (simp add: static_eval_state.simps)+ then
   have "\<forall>x \<omega>. \<rho> x = Some \<omega> \<longrightarrow> {|\<omega>|} \<subseteq> \<V> x" by (simp add: static_eval_env.simps)
   with `\<rho> x\<^sub>s = Some \<lbrace>prim.Right x\<^sub>r', \<rho>\<^sub>r\<rbrace>`
   have "^prim.Right x\<^sub>r' \<in> \<V> x\<^sub>s" by fastforce
@@ -167,17 +167,17 @@ proof -
 qed
 
 
-lemma accept_state_to_exp_let: "
+lemma static_eval_state_to_exp_let: "
   (\<V>, \<C>) \<Turnstile>\<^sub>\<sigma> \<langle>LET x = b in e; \<rho>; \<kappa>\<rangle> \<Longrightarrow> (\<V>, \<C>) \<Turnstile>\<^sub>e e
 "
 proof -
  assume "(\<V>, \<C>) \<Turnstile>\<^sub>\<sigma> \<langle>LET x = b in e; \<rho>; \<kappa>\<rangle>" then
- have "(\<V>, \<C>) \<Turnstile>\<^sub>e LET x = b in e" by (simp add: accept_state.simps) then
+ have "(\<V>, \<C>) \<Turnstile>\<^sub>e LET x = b in e" by (simp add: static_eval_state.simps) then
  show "(\<V>, \<C>) \<Turnstile>\<^sub>e e" by (rule static_eval.cases; auto)
 qed
 
 
-lemma accept_state_to_exp_let_app: "
+lemma static_eval_state_to_exp_let_app: "
  (\<V>, \<C>) \<Turnstile>\<^sub>\<sigma> \<langle>LET x = APP f x\<^sub>a in e; \<rho>; \<kappa>\<rangle> \<Longrightarrow> 
  \<rho> f = Some \<lbrace>Abs f' x\<^sub>p e\<^sub>b, \<rho>'\<rbrace> \<Longrightarrow>
  (\<V>, \<C>) \<Turnstile>\<^sub>e e\<^sub>b
@@ -186,14 +186,14 @@ lemma accept_state_to_exp_let_app: "
 proof -
   assume "\<rho> f = Some \<lbrace>Abs f' x\<^sub>p e\<^sub>b, \<rho>'\<rbrace>"
   assume "(\<V>, \<C>) \<Turnstile>\<^sub>\<sigma> \<langle>LET x = APP f x\<^sub>a in e; \<rho>; \<kappa>\<rangle>" then
-  have "(\<V>, \<C>) \<Turnstile>\<^sub>\<rho> \<rho>" by (simp add: accept_state.simps) then
+  have "(\<V>, \<C>) \<Turnstile>\<^sub>\<rho> \<rho>" by (simp add: static_eval_state.simps) then
   have "\<forall>x \<omega>. \<rho> x = Some \<omega> \<longrightarrow> {|\<omega>|} \<subseteq> \<V> x \<and> (\<V>, \<C>) \<Turnstile>\<^sub>\<omega> \<omega>" by (simp add: static_eval_env.simps)
   with `\<rho> f = Some \<lbrace>Abs f' x\<^sub>p e\<^sub>b, \<rho>'\<rbrace>`
   have "(\<V>, \<C>) \<Turnstile>\<^sub>\<omega> \<lbrace>Abs f' x\<^sub>p e\<^sub>b, \<rho>'\<rbrace>" by simp then
   show "(\<V>, \<C>) \<Turnstile>\<^sub>e e\<^sub>b" by (rule static_eval_value.cases; auto)
 qed
 
-lemma accept_state_to_env_result: "
+lemma static_eval_state_to_env_result: "
   (\<V>, \<C>) \<Turnstile>\<^sub>\<sigma> \<langle>RESULT x; \<rho>; \<langle>x\<^sub>\<kappa>,e\<^sub>\<kappa>,\<rho>\<^sub>\<kappa>\<rangle> # \<kappa>\<rangle> \<Longrightarrow> 
   \<rho> x = Some \<omega> \<Longrightarrow> 
   (\<V>, \<C>) \<Turnstile>\<^sub>\<rho> \<rho>\<^sub>\<kappa>(x\<^sub>\<kappa> \<mapsto> \<omega>)
@@ -202,7 +202,7 @@ proof
  assume "\<rho> x = Some \<omega> "
 
  assume "(\<V>, \<C>) \<Turnstile>\<^sub>\<sigma> \<langle>RESULT x; \<rho>; \<langle>x\<^sub>\<kappa>,e\<^sub>\<kappa>,\<rho>\<^sub>\<kappa>\<rangle> # \<kappa>\<rangle>" then
- have "(\<V>, \<C>) \<Turnstile>\<^sub>\<kappa> \<V> x \<Rrightarrow> \<langle>x\<^sub>\<kappa>,e\<^sub>\<kappa>,\<rho>\<^sub>\<kappa>\<rangle> # \<kappa>" and "(\<V>, \<C>) \<Turnstile>\<^sub>\<rho> \<rho>" by (rule accept_state.cases; auto)+
+ have "(\<V>, \<C>) \<Turnstile>\<^sub>\<kappa> \<V> x \<Rrightarrow> \<langle>x\<^sub>\<kappa>,e\<^sub>\<kappa>,\<rho>\<^sub>\<kappa>\<rangle> # \<kappa>" and "(\<V>, \<C>) \<Turnstile>\<^sub>\<rho> \<rho>" by (rule static_eval_state.cases; auto)+
 
  from `(\<V>, \<C>) \<Turnstile>\<^sub>\<rho> \<rho>` and `\<rho> x = Some \<omega>`
  have "{|\<omega>|} \<subseteq> \<V> x" "(\<V>, \<C>) \<Turnstile>\<^sub>\<omega> \<omega>" by (simp add: static_eval_env.simps)+
@@ -241,7 +241,7 @@ proof
 qed
 
 
-lemma accept_state_to_stack_result: "
+lemma static_eval_state_to_stack_result: "
   (\<V>, \<C>) \<Turnstile>\<^sub>\<sigma> \<langle>RESULT x; \<rho>; \<langle>x\<^sub>\<kappa>,e\<^sub>\<kappa>,\<rho>\<^sub>\<kappa>\<rangle> # \<kappa>\<rangle> \<Longrightarrow> 
   \<rho> x = Some \<omega> \<Longrightarrow> 
   (\<V>, \<C>) \<Turnstile>\<^sub>\<kappa> \<V> (\<lfloor>e\<^sub>\<kappa>\<rfloor>) \<Rrightarrow> \<kappa>
@@ -249,34 +249,34 @@ lemma accept_state_to_stack_result: "
 proof -
   assume "\<rho> x = Some \<omega>"
   assume "(\<V>, \<C>) \<Turnstile>\<^sub>\<sigma> \<langle>RESULT x; \<rho>; \<langle>x\<^sub>\<kappa>,e\<^sub>\<kappa>,\<rho>\<^sub>\<kappa>\<rangle> # \<kappa>\<rangle>" then
-  have "(\<V>, \<C>) \<Turnstile>\<^sub>\<kappa> \<V> x \<Rrightarrow> \<langle>x\<^sub>\<kappa>,e\<^sub>\<kappa>,\<rho>\<^sub>\<kappa>\<rangle> # \<kappa>" by (simp add: accept_state.simps) then
+  have "(\<V>, \<C>) \<Turnstile>\<^sub>\<kappa> \<V> x \<Rrightarrow> \<langle>x\<^sub>\<kappa>,e\<^sub>\<kappa>,\<rho>\<^sub>\<kappa>\<rangle> # \<kappa>" by (simp add: static_eval_state.simps) then
   show "(\<V>, \<C>) \<Turnstile>\<^sub>\<kappa> \<V> (\<lfloor>e\<^sub>\<kappa>\<rfloor>) \<Rrightarrow> \<kappa>" by (rule static_eval_stack.cases; auto)
 qed
 
 
-lemma accept_state_to_state_result: "
+lemma static_eval_state_to_state_result: "
   (\<V>, \<C>) \<Turnstile>\<^sub>\<sigma> \<langle>RESULT x; \<rho>; \<langle>x\<^sub>\<kappa>,e\<^sub>\<kappa>,\<rho>\<^sub>\<kappa>\<rangle> # \<kappa>\<rangle> \<Longrightarrow> 
   \<rho> x = Some \<omega> \<Longrightarrow> 
   (\<V>, \<C>) \<Turnstile>\<^sub>\<sigma> \<langle>e\<^sub>\<kappa>; \<rho>\<^sub>\<kappa>(x\<^sub>\<kappa> \<mapsto> \<omega>); \<kappa>\<rangle>
 "
 proof
   assume "\<rho> x = Some \<omega>" "(\<V>, \<C>) \<Turnstile>\<^sub>\<sigma> \<langle>RESULT x; \<rho>; \<langle>x\<^sub>\<kappa>,e\<^sub>\<kappa>,\<rho>\<^sub>\<kappa>\<rangle> # \<kappa>\<rangle>" then
-  show "(\<V>, \<C>) \<Turnstile>\<^sub>\<rho> \<rho>\<^sub>\<kappa>(x\<^sub>\<kappa> \<mapsto> \<omega>)" by (blast intro: accept_state_to_env_result)
+  show "(\<V>, \<C>) \<Turnstile>\<^sub>\<rho> \<rho>\<^sub>\<kappa>(x\<^sub>\<kappa> \<mapsto> \<omega>)" by (blast intro: static_eval_state_to_env_result)
 
   with `(\<V>, \<C>) \<Turnstile>\<^sub>\<sigma> \<langle>RESULT x; \<rho>; \<langle>x\<^sub>\<kappa>,e\<^sub>\<kappa>,\<rho>\<^sub>\<kappa>\<rangle> # \<kappa>\<rangle>`
-  show "(\<V>, \<C>) \<Turnstile>\<^sub>e e\<^sub>\<kappa>" by (blast intro: accept_state_to_exp_result)
+  show "(\<V>, \<C>) \<Turnstile>\<^sub>e e\<^sub>\<kappa>" by (blast intro: static_eval_state_to_exp_result)
 
   with `\<rho> x = Some \<omega>` `(\<V>, \<C>) \<Turnstile>\<^sub>\<sigma> \<langle>RESULT x; \<rho>; \<langle>x\<^sub>\<kappa>,e\<^sub>\<kappa>,\<rho>\<^sub>\<kappa>\<rangle> # \<kappa>\<rangle>`
-  show "(\<V>, \<C>) \<Turnstile>\<^sub>\<kappa> \<V> (\<lfloor>e\<^sub>\<kappa>\<rfloor>) \<Rrightarrow> \<kappa>" by (blast intro: accept_state_to_stack_result)
+  show "(\<V>, \<C>) \<Turnstile>\<^sub>\<kappa> \<V> (\<lfloor>e\<^sub>\<kappa>\<rfloor>) \<Rrightarrow> \<kappa>" by (blast intro: static_eval_state_to_stack_result)
 qed
 
 
-lemma accept_state_to_env_let_unit: "
+lemma static_eval_state_to_env_let_unit: "
   (\<V>, \<C>) \<Turnstile>\<^sub>\<sigma> \<langle>LET x = \<lparr>\<rparr> in e; \<rho>; \<kappa>\<rangle> \<Longrightarrow> (\<V>, \<C>) \<Turnstile>\<^sub>\<rho> \<rho>(x \<mapsto> \<lbrace>\<rbrace>)
 "
 proof
   assume "(\<V>, \<C>) \<Turnstile>\<^sub>\<sigma> \<langle>LET x = \<lparr>\<rparr> in e; \<rho>; \<kappa>\<rangle>" then 
-  have "(\<V>, \<C>) \<Turnstile>\<^sub>e LET x = \<lparr>\<rparr> in e" "(\<V>, \<C>) \<Turnstile>\<^sub>\<rho> \<rho>" by (simp add: accept_state.simps)+ 
+  have "(\<V>, \<C>) \<Turnstile>\<^sub>e LET x = \<lparr>\<rparr> in e" "(\<V>, \<C>) \<Turnstile>\<^sub>\<rho> \<rho>" by (simp add: static_eval_state.simps)+ 
 
   from `(\<V>, \<C>) \<Turnstile>\<^sub>e LET x = \<lparr>\<rparr> in e`
   have "{^\<lparr>\<rparr>} \<subseteq> \<V> x" by (rule static_eval.cases; auto)+
@@ -308,23 +308,23 @@ proof
 qed
 
 
-lemma accept_state_to_stack_let: "
+lemma static_eval_state_to_stack_let: "
   (\<V>, \<C>) \<Turnstile>\<^sub>\<sigma> \<langle>LET x = b in e; \<rho>; \<kappa>\<rangle> \<Longrightarrow> (\<V>, \<C>) \<Turnstile>\<^sub>\<kappa> \<V> (\<lfloor>e\<rfloor>) \<Rrightarrow> \<kappa>
 "
-by (erule accept_state.cases; auto)
+by (erule static_eval_state.cases; auto)
 
-lemma accept_state_to_state_let_unit: "
+lemma static_eval_state_to_state_let_unit: "
   (\<V>, \<C>) \<Turnstile>\<^sub>\<sigma> \<langle>LET x = \<lparr>\<rparr> in e; \<rho>; \<kappa>\<rangle> \<Longrightarrow> (\<V>, \<C>) \<Turnstile>\<^sub>\<sigma> \<langle>e; \<rho>(x \<mapsto> \<lbrace>\<rbrace>); \<kappa>\<rangle>
 "
 proof
   assume "(\<V>, \<C>) \<Turnstile>\<^sub>\<sigma> \<langle>LET x = \<lparr>\<rparr> in e; \<rho>; \<kappa>\<rangle>" then
-  show "(\<V>, \<C>) \<Turnstile>\<^sub>e e" by (auto simp: accept_state_to_exp_let)
+  show "(\<V>, \<C>) \<Turnstile>\<^sub>e e" by (auto simp: static_eval_state_to_exp_let)
 
   from `(\<V>, \<C>) \<Turnstile>\<^sub>\<sigma> \<langle>LET x = \<lparr>\<rparr> in e; \<rho>; \<kappa>\<rangle>` 
-  show "(\<V>, \<C>) \<Turnstile>\<^sub>\<rho> \<rho>(x \<mapsto> \<lbrace>\<rbrace>)" by (auto simp: accept_state_to_env_let_unit)
+  show "(\<V>, \<C>) \<Turnstile>\<^sub>\<rho> \<rho>(x \<mapsto> \<lbrace>\<rbrace>)" by (auto simp: static_eval_state_to_env_let_unit)
 
   from `(\<V>, \<C>) \<Turnstile>\<^sub>\<sigma> \<langle>LET x = \<lparr>\<rparr> in e; \<rho>; \<kappa>\<rangle>` 
-  show "(\<V>, \<C>) \<Turnstile>\<^sub>\<kappa> \<V> (\<lfloor>e\<rfloor>) \<Rrightarrow> \<kappa>" by (auto simp: accept_state_to_stack_let)
+  show "(\<V>, \<C>) \<Turnstile>\<^sub>\<kappa> \<V> (\<lfloor>e\<rfloor>) \<Rrightarrow> \<kappa>" by (auto simp: static_eval_state_to_stack_let)
 
 qed
 
@@ -333,12 +333,12 @@ lemma static_eval_to_value_let_prim: "
 "
 by (erule static_eval.cases; auto; rule; auto)
 
-lemma accept_state_to_env_let_prim: "
+lemma static_eval_state_to_env_let_prim: "
   (\<V>, \<C>) \<Turnstile>\<^sub>\<sigma> \<langle>LET x = Prim p in e; \<rho>; \<kappa>\<rangle> \<Longrightarrow> (\<V>, \<C>) \<Turnstile>\<^sub>\<rho> \<rho>(x \<mapsto> \<lbrace>p, \<rho>\<rbrace>)
 "
 proof
   assume "(\<V>, \<C>) \<Turnstile>\<^sub>\<sigma> \<langle>LET x = Prim p in e; \<rho>; \<kappa>\<rangle> " then 
-  have "(\<V>, \<C>) \<Turnstile>\<^sub>e LET x = Prim p in e" "(\<V>, \<C>) \<Turnstile>\<^sub>\<rho> \<rho>" by (simp add: accept_state.simps)+ then
+  have "(\<V>, \<C>) \<Turnstile>\<^sub>e LET x = Prim p in e" "(\<V>, \<C>) \<Turnstile>\<^sub>\<rho> \<rho>" by (simp add: static_eval_state.simps)+ then
   have "(\<V>, \<C>) \<Turnstile>\<^sub>\<omega> \<lbrace>p, \<rho>\<rbrace>" by (simp add: static_eval_to_value_let_prim)
 
   from `(\<V>, \<C>) \<Turnstile>\<^sub>e LET x = Prim p in e`
@@ -367,23 +367,23 @@ proof
   show "\<forall>x' \<omega>'. (\<rho>(x \<mapsto> \<lbrace>p, \<rho>\<rbrace>)) x' = Some \<omega>' \<longrightarrow> {|\<omega>'|} \<subseteq> \<V> x' \<and> (\<V>, \<C>) \<Turnstile>\<^sub>\<omega> \<omega>'" by auto
 qed
 
-lemma accept_state_to_state_let_prim: "
+lemma static_eval_state_to_state_let_prim: "
   (\<V>, \<C>) \<Turnstile>\<^sub>\<sigma> \<langle>LET x = Prim p in e; \<rho>; \<kappa>\<rangle> \<Longrightarrow> (\<V>, \<C>) \<Turnstile>\<^sub>\<sigma> \<langle>e; \<rho>(x \<mapsto> \<lbrace>p, \<rho>\<rbrace>); \<kappa>\<rangle>
 "
 proof
   assume "(\<V>, \<C>) \<Turnstile>\<^sub>\<sigma> \<langle>LET x = Prim p in e; \<rho>; \<kappa>\<rangle>" then
-  show "(\<V>, \<C>) \<Turnstile>\<^sub>e e" by (auto simp: accept_state_to_exp_let)
+  show "(\<V>, \<C>) \<Turnstile>\<^sub>e e" by (auto simp: static_eval_state_to_exp_let)
 
   from `(\<V>, \<C>) \<Turnstile>\<^sub>\<sigma> \<langle>LET x = Prim p in e; \<rho>; \<kappa>\<rangle>` 
-  show "(\<V>, \<C>) \<Turnstile>\<^sub>\<kappa> \<V> (\<lfloor>e\<rfloor>) \<Rrightarrow> \<kappa>" by (auto simp: accept_state_to_stack_let)
+  show "(\<V>, \<C>) \<Turnstile>\<^sub>\<kappa> \<V> (\<lfloor>e\<rfloor>) \<Rrightarrow> \<kappa>" by (auto simp: static_eval_state_to_stack_let)
 
   from `(\<V>, \<C>) \<Turnstile>\<^sub>\<sigma> \<langle>LET x = Prim p in e; \<rho>; \<kappa>\<rangle>` 
-  show "(\<V>, \<C>) \<Turnstile>\<^sub>\<rho> \<rho>(x \<mapsto> \<lbrace>p, \<rho>\<rbrace>)" by (auto simp: accept_state_to_env_let_prim)
+  show "(\<V>, \<C>) \<Turnstile>\<^sub>\<rho> \<rho>(x \<mapsto> \<lbrace>p, \<rho>\<rbrace>)" by (auto simp: static_eval_state_to_env_let_prim)
 
 qed
 
 
-lemma accept_state_to_env_let_case_left: "
+lemma static_eval_state_to_env_let_case_left: "
   (\<V>, \<C>) \<Turnstile>\<^sub>\<sigma> \<langle>LET x = CASE x\<^sub>s LEFT x\<^sub>l |> e\<^sub>l RIGHT x\<^sub>r |> e\<^sub>r in e; \<rho>; \<kappa>\<rangle> \<Longrightarrow> 
   \<rho> x\<^sub>s = Some \<lbrace>prim.Left x\<^sub>l', \<rho>\<^sub>l\<rbrace> \<Longrightarrow> \<rho>\<^sub>l x\<^sub>l' = Some \<omega>\<^sub>l \<Longrightarrow> 
   (\<V>, \<C>) \<Turnstile>\<^sub>\<rho> \<rho>(x\<^sub>l \<mapsto> \<omega>\<^sub>l)
@@ -392,7 +392,7 @@ lemma accept_state_to_env_let_case_left: "
 proof
   assume "\<rho> x\<^sub>s = Some \<lbrace>prim.Left x\<^sub>l', \<rho>\<^sub>l\<rbrace>" "\<rho>\<^sub>l x\<^sub>l' = Some \<omega>\<^sub>l"
   assume "(\<V>, \<C>) \<Turnstile>\<^sub>\<sigma> \<langle>LET x = CASE x\<^sub>s LEFT x\<^sub>l |> e\<^sub>l RIGHT x\<^sub>r |> e\<^sub>r in e; \<rho>; \<kappa>\<rangle>" then 
-  have "(\<V>, \<C>) \<Turnstile>\<^sub>e LET x = CASE x\<^sub>s LEFT x\<^sub>l |> e\<^sub>l RIGHT x\<^sub>r |> e\<^sub>r in e" "(\<V>, \<C>) \<Turnstile>\<^sub>\<rho> \<rho>" by (simp add: accept_state.simps)+
+  have "(\<V>, \<C>) \<Turnstile>\<^sub>e LET x = CASE x\<^sub>s LEFT x\<^sub>l |> e\<^sub>l RIGHT x\<^sub>r |> e\<^sub>r in e" "(\<V>, \<C>) \<Turnstile>\<^sub>\<rho> \<rho>" by (simp add: static_eval_state.simps)+
 
   from `(\<V>, \<C>) \<Turnstile>\<^sub>\<rho> \<rho>` `\<rho> x\<^sub>s = Some \<lbrace>prim.Left x\<^sub>l', \<rho>\<^sub>l\<rbrace>`
   have "(\<V>, \<C>) \<Turnstile>\<^sub>\<omega> \<lbrace>prim.Left x\<^sub>l', \<rho>\<^sub>l\<rbrace>" by (blast intro: static_eval_env.cases) then
@@ -430,7 +430,7 @@ proof
 qed
 
 
-lemma accept_state_to_stack_let_case_left: "
+lemma static_eval_state_to_stack_let_case_left: "
   (\<V>, \<C>) \<Turnstile>\<^sub>\<sigma> \<langle>LET x = CASE x\<^sub>s LEFT x\<^sub>l |> e\<^sub>l RIGHT x\<^sub>r |> e\<^sub>r in e; \<rho>; \<kappa>\<rangle> \<Longrightarrow>
   \<rho> x\<^sub>s = Some \<lbrace>prim.Left x\<^sub>l', \<rho>\<^sub>l\<rbrace> \<Longrightarrow> \<rho>\<^sub>l x\<^sub>l' = Some \<omega>\<^sub>l \<Longrightarrow> 
   (\<V>, \<C>) \<Turnstile>\<^sub>\<kappa> \<V> (\<lfloor>e\<^sub>l\<rfloor>) \<Rrightarrow> \<langle>x,e,\<rho>\<rangle> # \<kappa>
@@ -441,7 +441,7 @@ proof
   assume "\<rho> x\<^sub>s = Some \<lbrace>prim.Left x\<^sub>l', \<rho>\<^sub>l\<rbrace>" "\<rho>\<^sub>l x\<^sub>l' = Some \<omega>\<^sub>l"
 
   from `(\<V>, \<C>) \<Turnstile>\<^sub>\<sigma> \<langle>LET x = CASE x\<^sub>s LEFT x\<^sub>l |> e\<^sub>l RIGHT x\<^sub>r |> e\<^sub>r in e;\<rho>;\<kappa>\<rangle>`
-  have "(\<V>, \<C>) \<Turnstile>\<^sub>e LET x = CASE x\<^sub>s LEFT x\<^sub>l |> e\<^sub>l RIGHT x\<^sub>r |> e\<^sub>r in e" "(\<V>, \<C>) \<Turnstile>\<^sub>\<rho> \<rho>" by (blast intro: accept_state.cases)+
+  have "(\<V>, \<C>) \<Turnstile>\<^sub>e LET x = CASE x\<^sub>s LEFT x\<^sub>l |> e\<^sub>l RIGHT x\<^sub>r |> e\<^sub>r in e" "(\<V>, \<C>) \<Turnstile>\<^sub>\<rho> \<rho>" by (blast intro: static_eval_state.cases)+
   
   from `(\<V>, \<C>) \<Turnstile>\<^sub>\<rho> \<rho>` `\<rho> x\<^sub>s = Some \<lbrace>prim.Left x\<^sub>l', \<rho>\<^sub>l\<rbrace>`
   have " | \<lbrace>prim.Left x\<^sub>l', \<rho>\<^sub>l\<rbrace> | \<in> \<V> x\<^sub>s" by (blast intro: static_eval_env.cases) then
@@ -457,18 +457,18 @@ proof
   qed
 
   from `(\<V>, \<C>) \<Turnstile>\<^sub>\<sigma> \<langle>LET x = CASE x\<^sub>s LEFT x\<^sub>l |> e\<^sub>l RIGHT x\<^sub>r |> e\<^sub>r in e;\<rho>;\<kappa>\<rangle>`
-  show "(\<V>, \<C>) \<Turnstile>\<^sub>e e" by (blast intro: accept_state_to_exp_let)
+  show "(\<V>, \<C>) \<Turnstile>\<^sub>e e" by (blast intro: static_eval_state_to_exp_let)
 
   from `(\<V>, \<C>) \<Turnstile>\<^sub>\<sigma> \<langle>LET x = CASE x\<^sub>s LEFT x\<^sub>l |> e\<^sub>l RIGHT x\<^sub>r |> e\<^sub>r in e;\<rho>;\<kappa>\<rangle>`
-  show "(\<V>, \<C>) \<Turnstile>\<^sub>\<rho> \<rho>" by (blast intro: accept_state.cases)
+  show "(\<V>, \<C>) \<Turnstile>\<^sub>\<rho> \<rho>" by (blast intro: static_eval_state.cases)
 
   from `(\<V>, \<C>) \<Turnstile>\<^sub>\<sigma> \<langle>LET x = CASE x\<^sub>s LEFT x\<^sub>l |> e\<^sub>l RIGHT x\<^sub>r |> e\<^sub>r in e;\<rho>;\<kappa>\<rangle>`
-  show "(\<V>, \<C>) \<Turnstile>\<^sub>\<kappa> \<V> (\<lfloor>e\<rfloor>) \<Rrightarrow> \<kappa>" by (blast intro: accept_state_to_stack_let)
+  show "(\<V>, \<C>) \<Turnstile>\<^sub>\<kappa> \<V> (\<lfloor>e\<rfloor>) \<Rrightarrow> \<kappa>" by (blast intro: static_eval_state_to_stack_let)
   
 qed
 
 
-lemma accept_state_to_state_let_case_left: "
+lemma static_eval_state_to_state_let_case_left: "
   (\<V>, \<C>) \<Turnstile>\<^sub>\<sigma> \<langle>LET x = CASE x\<^sub>s LEFT x\<^sub>l |> e\<^sub>l RIGHT x\<^sub>r |> e\<^sub>r in e; \<rho>; \<kappa>\<rangle> \<Longrightarrow> 
   \<rho> x\<^sub>s = Some \<lbrace>prim.Left x\<^sub>l', \<rho>\<^sub>l\<rbrace> \<Longrightarrow> 
   \<rho>\<^sub>l x\<^sub>l' = Some \<omega>\<^sub>l \<Longrightarrow> 
@@ -476,20 +476,20 @@ lemma accept_state_to_state_let_case_left: "
 "
 proof
   assume "(\<V>, \<C>) \<Turnstile>\<^sub>\<sigma> \<langle>LET x = CASE x\<^sub>s LEFT x\<^sub>l |> e\<^sub>l RIGHT x\<^sub>r |> e\<^sub>r in e; \<rho>; \<kappa>\<rangle>" and "\<rho> x\<^sub>s = Some \<lbrace>prim.Left x\<^sub>l', \<rho>\<^sub>l\<rbrace>" then
-  show "(\<V>, \<C>) \<Turnstile>\<^sub>e e\<^sub>l" by (simp add: accept_state_to_exp_let_case_left)
+  show "(\<V>, \<C>) \<Turnstile>\<^sub>e e\<^sub>l" by (simp add: static_eval_state_to_exp_let_case_left)
 
   assume "\<rho>\<^sub>l x\<^sub>l' = Some \<omega>\<^sub>l"
   with `(\<V>, \<C>) \<Turnstile>\<^sub>\<sigma> \<langle>LET x = CASE x\<^sub>s LEFT x\<^sub>l |> e\<^sub>l RIGHT x\<^sub>r |> e\<^sub>r in e; \<rho>; \<kappa>\<rangle>` and `\<rho> x\<^sub>s = Some \<lbrace>prim.Left x\<^sub>l', \<rho>\<^sub>l\<rbrace>` 
-  show "(\<V>, \<C>) \<Turnstile>\<^sub>\<rho> \<rho>(x\<^sub>l \<mapsto> \<omega>\<^sub>l)" by (simp add: accept_state_to_env_let_case_left)
+  show "(\<V>, \<C>) \<Turnstile>\<^sub>\<rho> \<rho>(x\<^sub>l \<mapsto> \<omega>\<^sub>l)" by (simp add: static_eval_state_to_env_let_case_left)
 
   from `\<rho>\<^sub>l x\<^sub>l' = Some \<omega>\<^sub>l`  
   and `(\<V>, \<C>) \<Turnstile>\<^sub>\<sigma> \<langle>LET x = CASE x\<^sub>s LEFT x\<^sub>l |> e\<^sub>l RIGHT x\<^sub>r |> e\<^sub>r in e; \<rho>; \<kappa>\<rangle>` 
   and `\<rho> x\<^sub>s = Some \<lbrace>prim.Left x\<^sub>l', \<rho>\<^sub>l\<rbrace>` 
-  show "(\<V>, \<C>) \<Turnstile>\<^sub>\<kappa> \<V> (\<lfloor>e\<^sub>l\<rfloor>) \<Rrightarrow> \<langle>x,e,\<rho>\<rangle> # \<kappa>" by (simp add: accept_state_to_stack_let_case_left)
+  show "(\<V>, \<C>) \<Turnstile>\<^sub>\<kappa> \<V> (\<lfloor>e\<^sub>l\<rfloor>) \<Rrightarrow> \<langle>x,e,\<rho>\<rangle> # \<kappa>" by (simp add: static_eval_state_to_stack_let_case_left)
 qed
 
 
-lemma accept_state_to_env_let_case_right: "
+lemma static_eval_state_to_env_let_case_right: "
   (\<V>, \<C>) \<Turnstile>\<^sub>\<sigma> \<langle>LET x = CASE x\<^sub>s LEFT x\<^sub>l |> e\<^sub>l RIGHT x\<^sub>r |> e\<^sub>r in e; \<rho>; \<kappa>\<rangle> \<Longrightarrow> 
   \<rho> x\<^sub>s = Some \<lbrace>prim.Right x\<^sub>r', \<rho>\<^sub>r\<rbrace> \<Longrightarrow> \<rho>\<^sub>r x\<^sub>r' = Some \<omega>\<^sub>r \<Longrightarrow> 
   (\<V>, \<C>) \<Turnstile>\<^sub>\<rho> \<rho>(x\<^sub>r \<mapsto> \<omega>\<^sub>r)
@@ -498,7 +498,7 @@ lemma accept_state_to_env_let_case_right: "
 proof
   assume "\<rho> x\<^sub>s = Some \<lbrace>prim.Right x\<^sub>r', \<rho>\<^sub>r\<rbrace>" "\<rho>\<^sub>r x\<^sub>r' = Some \<omega>\<^sub>r"
   assume "(\<V>, \<C>) \<Turnstile>\<^sub>\<sigma> \<langle>LET x = CASE x\<^sub>s LEFT x\<^sub>l |> e\<^sub>l RIGHT x\<^sub>r |> e\<^sub>r in e; \<rho>; \<kappa>\<rangle>" then 
-  have "(\<V>, \<C>) \<Turnstile>\<^sub>e LET x = CASE x\<^sub>s LEFT x\<^sub>l |> e\<^sub>l RIGHT x\<^sub>r |> e\<^sub>r in e" "(\<V>, \<C>) \<Turnstile>\<^sub>\<rho> \<rho>" by (simp add: accept_state.simps)+
+  have "(\<V>, \<C>) \<Turnstile>\<^sub>e LET x = CASE x\<^sub>s LEFT x\<^sub>l |> e\<^sub>l RIGHT x\<^sub>r |> e\<^sub>r in e" "(\<V>, \<C>) \<Turnstile>\<^sub>\<rho> \<rho>" by (simp add: static_eval_state.simps)+
 
   from `(\<V>, \<C>) \<Turnstile>\<^sub>\<rho> \<rho>` `\<rho> x\<^sub>s = Some \<lbrace>prim.Right x\<^sub>r', \<rho>\<^sub>r\<rbrace>`
   have "(\<V>, \<C>) \<Turnstile>\<^sub>\<omega> \<lbrace>prim.Right x\<^sub>r', \<rho>\<^sub>r\<rbrace>" by (blast intro: static_eval_env.cases) then
@@ -535,7 +535,7 @@ proof
   show "\<forall>x' \<omega>'. (\<rho>(x\<^sub>r \<mapsto> \<omega>\<^sub>r)) x' = Some \<omega>' \<longrightarrow> {|\<omega>'|} \<subseteq> \<V> x' \<and> (\<V>, \<C>) \<Turnstile>\<^sub>\<omega> \<omega>'" by auto
 qed
 
-lemma accept_state_to_stack_let_case_right: "
+lemma static_eval_state_to_stack_let_case_right: "
   (\<V>, \<C>) \<Turnstile>\<^sub>\<sigma>  \<langle>LET x = CASE x\<^sub>s LEFT x\<^sub>l |> e\<^sub>l RIGHT x\<^sub>r |> e\<^sub>r in e; \<rho>; \<kappa>\<rangle> \<Longrightarrow>
   \<rho> x\<^sub>s = Some \<lbrace>prim.Right x\<^sub>r', \<rho>\<^sub>r\<rbrace> \<Longrightarrow> \<rho>\<^sub>r x\<^sub>r' = Some \<omega>\<^sub>r \<Longrightarrow> 
   (\<V>, \<C>) \<Turnstile>\<^sub>\<kappa>  \<V> (\<lfloor>e\<^sub>r\<rfloor>) \<Rrightarrow> \<langle>x,e,\<rho>\<rangle> # \<kappa>
@@ -546,7 +546,7 @@ proof
   assume "\<rho> x\<^sub>s = Some \<lbrace>prim.Right x\<^sub>r', \<rho>\<^sub>r\<rbrace>" "\<rho>\<^sub>r x\<^sub>r' = Some \<omega>\<^sub>r"
 
   from `(\<V>, \<C>) \<Turnstile>\<^sub>\<sigma> \<langle>LET x = CASE x\<^sub>s LEFT x\<^sub>l |> e\<^sub>l RIGHT x\<^sub>r |> e\<^sub>r in e;\<rho>;\<kappa>\<rangle>`
-  have "(\<V>, \<C>) \<Turnstile>\<^sub>e LET x = CASE x\<^sub>s LEFT x\<^sub>l |> e\<^sub>l RIGHT x\<^sub>r |> e\<^sub>r in e" "(\<V>, \<C>) \<Turnstile>\<^sub>\<rho> \<rho>" by (blast intro: accept_state.cases)+
+  have "(\<V>, \<C>) \<Turnstile>\<^sub>e LET x = CASE x\<^sub>s LEFT x\<^sub>l |> e\<^sub>l RIGHT x\<^sub>r |> e\<^sub>r in e" "(\<V>, \<C>) \<Turnstile>\<^sub>\<rho> \<rho>" by (blast intro: static_eval_state.cases)+
   
   from `(\<V>, \<C>) \<Turnstile>\<^sub>\<rho> \<rho>` `\<rho> x\<^sub>s = Some \<lbrace>prim.Right x\<^sub>r', \<rho>\<^sub>r\<rbrace>`
   have " | \<lbrace>prim.Right x\<^sub>r', \<rho>\<^sub>r\<rbrace> | \<in> \<V> x\<^sub>s" by (blast intro: static_eval_env.cases) then
@@ -562,37 +562,37 @@ proof
   qed
 
   from `(\<V>, \<C>) \<Turnstile>\<^sub>\<sigma> \<langle>LET x = CASE x\<^sub>s LEFT x\<^sub>l |> e\<^sub>l RIGHT x\<^sub>r |> e\<^sub>r in e;\<rho>;\<kappa>\<rangle>`
-  show "(\<V>, \<C>) \<Turnstile>\<^sub>e e" by (blast intro: accept_state_to_exp_let)
+  show "(\<V>, \<C>) \<Turnstile>\<^sub>e e" by (blast intro: static_eval_state_to_exp_let)
 
   from `(\<V>, \<C>) \<Turnstile>\<^sub>\<sigma> \<langle>LET x = CASE x\<^sub>s LEFT x\<^sub>l |> e\<^sub>l RIGHT x\<^sub>r |> e\<^sub>r in e;\<rho>;\<kappa>\<rangle>`
-  show "(\<V>, \<C>) \<Turnstile>\<^sub>\<rho> \<rho>" by (blast intro: accept_state.cases)
+  show "(\<V>, \<C>) \<Turnstile>\<^sub>\<rho> \<rho>" by (blast intro: static_eval_state.cases)
 
   from `(\<V>, \<C>) \<Turnstile>\<^sub>\<sigma> \<langle>LET x = CASE x\<^sub>s LEFT x\<^sub>l |> e\<^sub>l RIGHT x\<^sub>r |> e\<^sub>r in e;\<rho>;\<kappa>\<rangle>`
-  show "(\<V>, \<C>) \<Turnstile>\<^sub>\<kappa> \<V> (\<lfloor>e\<rfloor>) \<Rrightarrow> \<kappa>" by (blast intro: accept_state_to_stack_let)
+  show "(\<V>, \<C>) \<Turnstile>\<^sub>\<kappa> \<V> (\<lfloor>e\<rfloor>) \<Rrightarrow> \<kappa>" by (blast intro: static_eval_state_to_stack_let)
   
 qed
 
-lemma accept_state_to_state_let_case_right: "
+lemma static_eval_state_to_state_let_case_right: "
   (\<V>, \<C>) \<Turnstile>\<^sub>\<sigma> \<langle>LET x = CASE x\<^sub>s LEFT x\<^sub>l |> e\<^sub>l RIGHT x\<^sub>r |> e\<^sub>r in e; \<rho>; \<kappa>\<rangle> \<Longrightarrow> 
   \<rho> x\<^sub>s = Some \<lbrace>prim.Right x\<^sub>r', \<rho>\<^sub>r\<rbrace> \<Longrightarrow> 
   \<rho>\<^sub>r x\<^sub>r' = Some \<omega>\<^sub>r \<Longrightarrow> (\<V>, \<C>) \<Turnstile>\<^sub>\<sigma> \<langle>e\<^sub>r; \<rho>(x\<^sub>r \<mapsto> \<omega>\<^sub>r); \<langle>x,e,\<rho>\<rangle> # \<kappa>\<rangle>
 "
 proof
   assume "(\<V>, \<C>) \<Turnstile>\<^sub>\<sigma> \<langle>LET x = CASE x\<^sub>s LEFT x\<^sub>l |> e\<^sub>l RIGHT x\<^sub>r |> e\<^sub>r in e; \<rho>; \<kappa>\<rangle>" and "\<rho> x\<^sub>s = Some \<lbrace>prim.Right x\<^sub>r', \<rho>\<^sub>r\<rbrace>" then
-  show "(\<V>, \<C>) \<Turnstile>\<^sub>e e\<^sub>r" by (simp add: accept_state_to_exp_let_case_right)
+  show "(\<V>, \<C>) \<Turnstile>\<^sub>e e\<^sub>r" by (simp add: static_eval_state_to_exp_let_case_right)
 
   assume "\<rho>\<^sub>r x\<^sub>r' = Some \<omega>\<^sub>r"
   with `(\<V>, \<C>) \<Turnstile>\<^sub>\<sigma> \<langle>LET x = CASE x\<^sub>s LEFT x\<^sub>l |> e\<^sub>l RIGHT x\<^sub>r |> e\<^sub>r in e; \<rho>; \<kappa>\<rangle>` and `\<rho> x\<^sub>s = Some \<lbrace>prim.Right x\<^sub>r', \<rho>\<^sub>r\<rbrace>` 
-  show "(\<V>, \<C>) \<Turnstile>\<^sub>\<rho> \<rho>(x\<^sub>r \<mapsto> \<omega>\<^sub>r)" by (simp add: accept_state_to_env_let_case_right)
+  show "(\<V>, \<C>) \<Turnstile>\<^sub>\<rho> \<rho>(x\<^sub>r \<mapsto> \<omega>\<^sub>r)" by (simp add: static_eval_state_to_env_let_case_right)
 
   from `\<rho>\<^sub>r x\<^sub>r' = Some \<omega>\<^sub>r`  
   and `(\<V>, \<C>) \<Turnstile>\<^sub>\<sigma> \<langle>LET x = CASE x\<^sub>s LEFT x\<^sub>l |> e\<^sub>l RIGHT x\<^sub>r |> e\<^sub>r in e; \<rho>; \<kappa>\<rangle>` 
   and `\<rho> x\<^sub>s = Some \<lbrace>prim.Right x\<^sub>r', \<rho>\<^sub>r\<rbrace>` 
-  show "(\<V>, \<C>) \<Turnstile>\<^sub>\<kappa> \<V> (\<lfloor>e\<^sub>r\<rfloor>) \<Rrightarrow> \<langle>x,e,\<rho>\<rangle> # \<kappa>" by (simp add: accept_state_to_stack_let_case_right)
+  show "(\<V>, \<C>) \<Turnstile>\<^sub>\<kappa> \<V> (\<lfloor>e\<^sub>r\<rfloor>) \<Rrightarrow> \<langle>x,e,\<rho>\<rangle> # \<kappa>" by (simp add: static_eval_state_to_stack_let_case_right)
 qed
 
 
-lemma accept_state_to_env_let_fst: "
+lemma static_eval_state_to_env_let_fst: "
   (\<V>, \<C>) \<Turnstile>\<^sub>\<sigma> \<langle>LET x = FST x\<^sub>p in e; \<rho>; \<kappa>\<rangle> \<Longrightarrow> 
   \<rho> x\<^sub>p = Some \<lbrace>prim.Pair x\<^sub>1 x\<^sub>2, \<rho>\<^sub>p\<rbrace> \<Longrightarrow> \<rho>\<^sub>p x\<^sub>1 = Some \<omega> \<Longrightarrow> 
   (\<V>, \<C>) \<Turnstile>\<^sub>\<rho> \<rho>(x \<mapsto> \<omega>)
@@ -600,9 +600,9 @@ lemma accept_state_to_env_let_fst: "
 proof
   assume "\<rho> x\<^sub>p = Some \<lbrace>prim.Pair x\<^sub>1 x\<^sub>2, \<rho>\<^sub>p\<rbrace>" and "\<rho>\<^sub>p x\<^sub>1 = Some \<omega>"
   assume "(\<V>, \<C>) \<Turnstile>\<^sub>\<sigma> \<langle>LET x = FST x\<^sub>p in e; \<rho>; \<kappa>\<rangle>" then
-  have "(\<V>, \<C>) \<Turnstile>\<^sub>e LET x = FST x\<^sub>p in e" "(\<V>, \<C>) \<Turnstile>\<^sub>\<rho> \<rho>" by (simp add: accept_state.simps)+
+  have "(\<V>, \<C>) \<Turnstile>\<^sub>e LET x = FST x\<^sub>p in e" "(\<V>, \<C>) \<Turnstile>\<^sub>\<rho> \<rho>" by (simp add: static_eval_state.simps)+
 
-  thm accept_state.simps
+  thm static_eval_state.simps
 
   from `(\<V>, \<C>) \<Turnstile>\<^sub>\<rho> \<rho>` `\<rho> x\<^sub>p = Some \<lbrace>prim.Pair x\<^sub>1 x\<^sub>2, \<rho>\<^sub>p\<rbrace>`
   have "(\<V>, \<C>) \<Turnstile>\<^sub>\<omega> \<lbrace>prim.Pair x\<^sub>1 x\<^sub>2, \<rho>\<^sub>p\<rbrace>" by (blast intro: static_eval_env.cases) then
@@ -640,32 +640,32 @@ qed
 
 
 
-lemma accept_state_to_state_let_fst: "
+lemma static_eval_state_to_state_let_fst: "
   (\<V>, \<C>) \<Turnstile>\<^sub>\<sigma> \<langle>LET x = FST x\<^sub>p in e; \<rho>; \<kappa>\<rangle> \<Longrightarrow>
   \<rho> x\<^sub>p = Some \<lbrace>prim.Pair x\<^sub>1 x\<^sub>2, \<rho>\<^sub>p\<rbrace> \<Longrightarrow> \<rho>\<^sub>p x\<^sub>1 = Some \<omega> \<Longrightarrow> 
   (\<V>, \<C>) \<Turnstile>\<^sub>\<sigma> \<langle>e; \<rho>(x \<mapsto> \<omega>); \<kappa>\<rangle>
 "
 proof
   assume "(\<V>, \<C>) \<Turnstile>\<^sub>\<sigma> \<langle>LET x = FST x\<^sub>p in e; \<rho>; \<kappa>\<rangle>" then
-  show "(\<V>, \<C>) \<Turnstile>\<^sub>e e" by (simp add: accept_state_to_exp_let)
+  show "(\<V>, \<C>) \<Turnstile>\<^sub>e e" by (simp add: static_eval_state_to_exp_let)
 
   assume "\<rho> x\<^sub>p = Some \<lbrace>prim.Pair x\<^sub>1 x\<^sub>2, \<rho>\<^sub>p\<rbrace>" and "\<rho>\<^sub>p x\<^sub>1 = Some \<omega>"
   with `(\<V>, \<C>) \<Turnstile>\<^sub>\<sigma> \<langle>LET x = FST x\<^sub>p in e; \<rho>; \<kappa>\<rangle>`
-  show "(\<V>, \<C>) \<Turnstile>\<^sub>\<rho> \<rho>(x \<mapsto> \<omega>)"  by (simp add: accept_state_to_env_let_fst)
+  show "(\<V>, \<C>) \<Turnstile>\<^sub>\<rho> \<rho>(x \<mapsto> \<omega>)"  by (simp add: static_eval_state_to_env_let_fst)
 
   from `\<rho> x\<^sub>p = Some \<lbrace>prim.Pair x\<^sub>1 x\<^sub>2, \<rho>\<^sub>p\<rbrace>` and `\<rho>\<^sub>p x\<^sub>1 = Some \<omega>`
   and `(\<V>, \<C>) \<Turnstile>\<^sub>\<sigma> \<langle>LET x = FST x\<^sub>p in e; \<rho>; \<kappa>\<rangle>`
-  show "(\<V>, \<C>) \<Turnstile>\<^sub>\<kappa> \<V> (\<lfloor>e\<rfloor>) \<Rrightarrow> \<kappa>" by (simp add: accept_state_to_stack_let)
+  show "(\<V>, \<C>) \<Turnstile>\<^sub>\<kappa> \<V> (\<lfloor>e\<rfloor>) \<Rrightarrow> \<kappa>" by (simp add: static_eval_state_to_stack_let)
 qed
 
 
-lemma accept_state_to_env_let_snd: "
+lemma static_eval_state_to_env_let_snd: "
   (\<V>, \<C>) \<Turnstile>\<^sub>\<sigma> \<langle>LET x = SND x\<^sub>p in e; \<rho>; \<kappa>\<rangle> \<Longrightarrow> \<rho> x\<^sub>p = Some \<lbrace>prim.Pair x\<^sub>1 x\<^sub>2, \<rho>\<^sub>p\<rbrace> \<Longrightarrow> \<rho>\<^sub>p x\<^sub>2 = Some \<omega> \<Longrightarrow> (\<V>, \<C>) \<Turnstile>\<^sub>\<rho> \<rho>(x \<mapsto> \<omega>)
 "
 proof
   assume "\<rho> x\<^sub>p = Some \<lbrace>prim.Pair x\<^sub>1 x\<^sub>2, \<rho>\<^sub>p\<rbrace>" and "\<rho>\<^sub>p x\<^sub>2 = Some \<omega>"
   assume "(\<V>, \<C>) \<Turnstile>\<^sub>\<sigma> \<langle>LET x = SND x\<^sub>p in e; \<rho>; \<kappa>\<rangle>" then
-  have "(\<V>, \<C>) \<Turnstile>\<^sub>e LET x = SND x\<^sub>p in e" "(\<V>, \<C>) \<Turnstile>\<^sub>\<rho> \<rho>" by (simp add: accept_state.simps)+
+  have "(\<V>, \<C>) \<Turnstile>\<^sub>e LET x = SND x\<^sub>p in e" "(\<V>, \<C>) \<Turnstile>\<^sub>\<rho> \<rho>" by (simp add: static_eval_state.simps)+
 
   from `(\<V>, \<C>) \<Turnstile>\<^sub>\<rho> \<rho>` `\<rho> x\<^sub>p = Some \<lbrace>prim.Pair x\<^sub>1 x\<^sub>2, \<rho>\<^sub>p\<rbrace>`
   have "(\<V>, \<C>) \<Turnstile>\<^sub>\<omega> \<lbrace>prim.Pair x\<^sub>1 x\<^sub>2, \<rho>\<^sub>p\<rbrace>" by (blast intro: static_eval_env.cases) then
@@ -703,26 +703,26 @@ proof
 qed
 
 
-lemma accept_state_to_state_let_snd: "
+lemma static_eval_state_to_state_let_snd: "
   (\<V>, \<C>) \<Turnstile>\<^sub>\<sigma> \<langle>LET x = SND x\<^sub>p in e; \<rho>; \<kappa>\<rangle> \<Longrightarrow>
   \<rho> x\<^sub>p = Some \<lbrace>prim.Pair x\<^sub>1 x\<^sub>2, \<rho>\<^sub>p\<rbrace> \<Longrightarrow> \<rho>\<^sub>p x\<^sub>2 = Some \<omega> \<Longrightarrow> 
   (\<V>, \<C>) \<Turnstile>\<^sub>\<sigma> \<langle>e; \<rho>(x \<mapsto> \<omega>); \<kappa>\<rangle>
 "
 proof
   assume "(\<V>, \<C>) \<Turnstile>\<^sub>\<sigma> \<langle>LET x = SND x\<^sub>p in e; \<rho>; \<kappa>\<rangle>" then
-  show "(\<V>, \<C>) \<Turnstile>\<^sub>e e" by (simp add: accept_state_to_exp_let)
+  show "(\<V>, \<C>) \<Turnstile>\<^sub>e e" by (simp add: static_eval_state_to_exp_let)
 
   assume "\<rho> x\<^sub>p = Some \<lbrace>prim.Pair x\<^sub>1 x\<^sub>2, \<rho>\<^sub>p\<rbrace>" and "\<rho>\<^sub>p x\<^sub>2 = Some \<omega>"
   with `(\<V>, \<C>) \<Turnstile>\<^sub>\<sigma> \<langle>LET x = SND x\<^sub>p in e; \<rho>; \<kappa>\<rangle>`
-  show "(\<V>, \<C>) \<Turnstile>\<^sub>\<rho> \<rho>(x \<mapsto> \<omega>)" by (simp add: accept_state_to_env_let_snd)
+  show "(\<V>, \<C>) \<Turnstile>\<^sub>\<rho> \<rho>(x \<mapsto> \<omega>)" by (simp add: static_eval_state_to_env_let_snd)
 
   from `\<rho> x\<^sub>p = Some \<lbrace>prim.Pair x\<^sub>1 x\<^sub>2, \<rho>\<^sub>p\<rbrace>` and `\<rho>\<^sub>p x\<^sub>2 = Some \<omega>`
   and `(\<V>, \<C>) \<Turnstile>\<^sub>\<sigma> \<langle>LET x = SND x\<^sub>p in e; \<rho>; \<kappa>\<rangle>`
-  show "(\<V>, \<C>) \<Turnstile>\<^sub>\<kappa> \<V> (\<lfloor>e\<rfloor>) \<Rrightarrow> \<kappa>" by (simp add: accept_state_to_stack_let)
+  show "(\<V>, \<C>) \<Turnstile>\<^sub>\<kappa> \<V> (\<lfloor>e\<rfloor>) \<Rrightarrow> \<kappa>" by (simp add: static_eval_state_to_stack_let)
 qed
 
 
-lemma accept_state_to_env_let_app: "
+lemma static_eval_state_to_env_let_app: "
   (\<V>, \<C>) \<Turnstile>\<^sub>\<sigma> \<langle>LET x = APP f x\<^sub>a in e; \<rho>; \<kappa>\<rangle> \<Longrightarrow> 
   \<rho> f = Some \<lbrace>Abs f\<^sub>l x\<^sub>l e\<^sub>l, \<rho>\<^sub>l\<rbrace> \<Longrightarrow> \<rho> x\<^sub>a = Some \<omega>\<^sub>a \<Longrightarrow> 
   (\<V>, \<C>) \<Turnstile>\<^sub>\<rho> \<rho>\<^sub>l(f\<^sub>l \<mapsto> \<lbrace>Abs f\<^sub>l x\<^sub>l e\<^sub>l, \<rho>\<^sub>l\<rbrace>, x\<^sub>l \<mapsto> \<omega>\<^sub>a)
@@ -730,7 +730,7 @@ lemma accept_state_to_env_let_app: "
 proof
   assume "\<rho> f = Some \<lbrace>Abs f\<^sub>l x\<^sub>l e\<^sub>l, \<rho>\<^sub>l\<rbrace>" "\<rho> x\<^sub>a = Some \<omega>\<^sub>a"
   assume "(\<V>, \<C>) \<Turnstile>\<^sub>\<sigma> \<langle>LET x = APP f x\<^sub>a in e; \<rho>; \<kappa>\<rangle>" then
-  have "(\<V>, \<C>) \<Turnstile>\<^sub>e LET x = APP f x\<^sub>a in e" "(\<V>, \<C>) \<Turnstile>\<^sub>\<rho> \<rho>" by (simp add: accept_state.simps)+
+  have "(\<V>, \<C>) \<Turnstile>\<^sub>e LET x = APP f x\<^sub>a in e" "(\<V>, \<C>) \<Turnstile>\<^sub>\<rho> \<rho>" by (simp add: static_eval_state.simps)+
 
   from `(\<V>, \<C>) \<Turnstile>\<^sub>\<rho> \<rho>` and `\<rho> x\<^sub>a = Some \<omega>\<^sub>a`
   have "{|\<omega>\<^sub>a|} \<subseteq> \<V> x\<^sub>a" "(\<V>, \<C>) \<Turnstile>\<^sub>\<omega> \<omega>\<^sub>a" by (blast intro: static_eval_env.cases)+
@@ -770,7 +770,7 @@ proof
 
 qed
 
-lemma accept_state_to_stack_let_app: "
+lemma static_eval_state_to_stack_let_app: "
   (\<V>, \<C>) \<Turnstile>\<^sub>\<sigma> \<langle>LET x = APP f x\<^sub>a in e; \<rho>; \<kappa>\<rangle> \<Longrightarrow> 
   \<rho> f = Some \<lbrace>Abs f' x\<^sub>p e\<^sub>b, \<rho>'\<rbrace> \<Longrightarrow> \<rho> x\<^sub>a = Some \<omega>\<^sub>a \<Longrightarrow> 
   (\<V>, \<C>) \<Turnstile>\<^sub>\<kappa> \<V> (\<lfloor>e\<^sub>b\<rfloor>) \<Rrightarrow> \<langle>x,e,\<rho>\<rangle> # \<kappa>
@@ -778,7 +778,7 @@ lemma accept_state_to_stack_let_app: "
 proof
   assume "\<rho> f = Some \<lbrace>Abs f' x\<^sub>p e\<^sub>b, \<rho>'\<rbrace>" and "\<rho> x\<^sub>a = Some \<omega>\<^sub>a"
   assume "(\<V>, \<C>) \<Turnstile>\<^sub>\<sigma> \<langle>LET x = APP f x\<^sub>a in e; \<rho>; \<kappa>\<rangle>" then
-  have "(\<V>, \<C>) \<Turnstile>\<^sub>e LET x = APP f x\<^sub>a in e"  "(\<V>, \<C>) \<Turnstile>\<^sub>\<rho> \<rho>" by (blast intro: accept_state.cases)+
+  have "(\<V>, \<C>) \<Turnstile>\<^sub>e LET x = APP f x\<^sub>a in e"  "(\<V>, \<C>) \<Turnstile>\<^sub>\<rho> \<rho>" by (blast intro: static_eval_state.cases)+
 
   from `(\<V>, \<C>) \<Turnstile>\<^sub>\<rho> \<rho>` and `\<rho> f = Some \<lbrace>Abs f' x\<^sub>p e\<^sub>b, \<rho>'\<rbrace>`
   have " {|\<lbrace>Abs f' x\<^sub>p e\<^sub>b, \<rho>'\<rbrace>|} \<subseteq> \<V> f" by (blast intro: static_eval_env.cases) then
@@ -794,34 +794,34 @@ proof
   qed
 
   from `(\<V>, \<C>) \<Turnstile>\<^sub>\<sigma> \<langle>LET x = APP f x\<^sub>a in e; \<rho>; \<kappa>\<rangle>`
-  show "(\<V>, \<C>) \<Turnstile>\<^sub>e e" by (blast intro: accept_state_to_exp_let)
+  show "(\<V>, \<C>) \<Turnstile>\<^sub>e e" by (blast intro: static_eval_state_to_exp_let)
 
   from `(\<V>, \<C>) \<Turnstile>\<^sub>\<sigma> \<langle>LET x = APP f x\<^sub>a in e; \<rho>; \<kappa>\<rangle>`
-  show "(\<V>, \<C>) \<Turnstile>\<^sub>\<rho> \<rho>" by (blast intro: accept_state.cases)
+  show "(\<V>, \<C>) \<Turnstile>\<^sub>\<rho> \<rho>" by (blast intro: static_eval_state.cases)
 
   from `(\<V>, \<C>) \<Turnstile>\<^sub>\<sigma> \<langle>LET x = APP f x\<^sub>a in e; \<rho>; \<kappa>\<rangle>`
-  show "(\<V>, \<C>) \<Turnstile>\<^sub>\<kappa> \<V> (\<lfloor>e\<rfloor>) \<Rrightarrow> \<kappa>" by (blast intro: accept_state_to_stack_let)
+  show "(\<V>, \<C>) \<Turnstile>\<^sub>\<kappa> \<V> (\<lfloor>e\<rfloor>) \<Rrightarrow> \<kappa>" by (blast intro: static_eval_state_to_stack_let)
 qed
 
 
-lemma accept_state_to_state_let_app: "
+lemma static_eval_state_to_state_let_app: "
   (\<V>, \<C>) \<Turnstile>\<^sub>\<sigma> \<langle>LET x = APP f x\<^sub>a in e; \<rho>; \<kappa>\<rangle> \<Longrightarrow>
   \<rho> f = Some \<lbrace>Abs f' x\<^sub>p e\<^sub>b, \<rho>'\<rbrace> \<Longrightarrow> \<rho> x\<^sub>a = Some \<omega>\<^sub>a \<Longrightarrow> 
   (\<V>, \<C>) \<Turnstile>\<^sub>\<sigma> \<langle>e\<^sub>b; \<rho>'(f' \<mapsto> \<lbrace>Abs f' x\<^sub>p e\<^sub>b, \<rho>'\<rbrace>, x\<^sub>p \<mapsto> \<omega>\<^sub>a); \<langle>x,e,\<rho>\<rangle> # \<kappa>\<rangle>
 "
 proof
   assume "(\<V>, \<C>) \<Turnstile>\<^sub>\<sigma> \<langle>LET x = APP f x\<^sub>a in e; \<rho>; \<kappa>\<rangle>" and "\<rho> f = Some \<lbrace>Abs f' x\<^sub>p e\<^sub>b, \<rho>'\<rbrace>" then
-  show "(\<V>, \<C>) \<Turnstile>\<^sub>e e\<^sub>b" by (blast intro: accept_state_to_exp_let_app)
+  show "(\<V>, \<C>) \<Turnstile>\<^sub>e e\<^sub>b" by (blast intro: static_eval_state_to_exp_let_app)
 
   assume "\<rho> x\<^sub>a = Some \<omega>\<^sub>a"
   with `(\<V>, \<C>) \<Turnstile>\<^sub>\<sigma> \<langle>LET x = APP f x\<^sub>a in e; \<rho>; \<kappa>\<rangle>` and `\<rho> f = Some \<lbrace>Abs f' x\<^sub>p e\<^sub>b, \<rho>'\<rbrace>`
-  show "(\<V>, \<C>) \<Turnstile>\<^sub>\<rho> \<rho>'(f' \<mapsto> \<lbrace>Abs f' x\<^sub>p e\<^sub>b, \<rho>'\<rbrace>, x\<^sub>p \<mapsto> \<omega>\<^sub>a)" by (blast intro: accept_state_to_env_let_app)
+  show "(\<V>, \<C>) \<Turnstile>\<^sub>\<rho> \<rho>'(f' \<mapsto> \<lbrace>Abs f' x\<^sub>p e\<^sub>b, \<rho>'\<rbrace>, x\<^sub>p \<mapsto> \<omega>\<^sub>a)" by (blast intro: static_eval_state_to_env_let_app)
 
   from `\<rho> x\<^sub>a = Some \<omega>\<^sub>a` and  `(\<V>, \<C>) \<Turnstile>\<^sub>\<sigma> \<langle>LET x = APP f x\<^sub>a in e; \<rho>; \<kappa>\<rangle>` and `\<rho> f = Some \<lbrace>Abs f' x\<^sub>p e\<^sub>b, \<rho>'\<rbrace>`
-  show "(\<V>, \<C>) \<Turnstile>\<^sub>\<kappa> \<V> (\<lfloor>e\<^sub>b\<rfloor>) \<Rrightarrow> \<langle>x,e,\<rho>\<rangle> # \<kappa>" by (blast intro: accept_state_to_stack_let_app)
+  show "(\<V>, \<C>) \<Turnstile>\<^sub>\<kappa> \<V> (\<lfloor>e\<^sub>b\<rfloor>) \<Rrightarrow> \<langle>x,e,\<rho>\<rangle> # \<kappa>" by (blast intro: static_eval_state_to_stack_let_app)
 qed
 
-theorem accept_state_preserved_under_step : "
+theorem static_eval_state_preserved_under_step : "
   \<lbrakk>
     (\<V>, \<C>) \<Turnstile>\<^sub>\<sigma> \<sigma>; 
     \<sigma> \<hookrightarrow> \<sigma>'
@@ -836,31 +836,31 @@ proof -
     case (Result \<rho> x \<omega> x\<^sub>\<kappa> e\<^sub>\<kappa> \<rho>\<^sub>\<kappa> \<kappa>)
     assume "\<sigma> = \<langle>RESULT x;\<rho>;\<langle>x\<^sub>\<kappa>,e\<^sub>\<kappa>,\<rho>\<^sub>\<kappa>\<rangle> # \<kappa>\<rangle>" and "\<sigma>' = \<langle>e\<^sub>\<kappa>;\<rho>\<^sub>\<kappa> ++ [x\<^sub>\<kappa> \<mapsto> \<omega>];\<kappa>\<rangle>" and "\<rho> x = Some \<omega>" 
     with `(\<V>, \<C>) \<Turnstile>\<^sub>\<sigma> \<sigma>`
-    show "(\<V>, \<C>) \<Turnstile>\<^sub>\<sigma> \<sigma>'" by (simp add: accept_state_to_state_result)
+    show "(\<V>, \<C>) \<Turnstile>\<^sub>\<sigma> \<sigma>'" by (simp add: static_eval_state_to_state_result)
   next
     case (Let_Unit x e \<rho> \<kappa>)
     assume "\<sigma> = \<langle>LET x = \<lparr>\<rparr> in e;\<rho>;\<kappa>\<rangle>" and "\<sigma>' = \<langle>e;\<rho> ++ [x \<mapsto> \<lbrace>\<rbrace>];\<kappa>\<rangle>"
     with `(\<V>, \<C>) \<Turnstile>\<^sub>\<sigma> \<sigma>`
-    show "(\<V>, \<C>) \<Turnstile>\<^sub>\<sigma> \<sigma>'" by (simp add: accept_state_to_state_let_unit)
+    show "(\<V>, \<C>) \<Turnstile>\<^sub>\<sigma> \<sigma>'" by (simp add: static_eval_state_to_state_let_unit)
   next
     case (Let_Prim x p e \<rho> \<kappa>)
     assume "\<sigma> = \<langle>LET x = Prim p in e;\<rho>;\<kappa>\<rangle>" and "\<sigma>' = \<langle>e;\<rho> ++ [x \<mapsto> \<lbrace>p, \<rho>\<rbrace>];\<kappa>\<rangle>"
     with `(\<V>, \<C>) \<Turnstile>\<^sub>\<sigma> \<sigma>`
-    show "(\<V>, \<C>) \<Turnstile>\<^sub>\<sigma> \<sigma>'" by (simp add: accept_state_to_state_let_prim)
+    show "(\<V>, \<C>) \<Turnstile>\<^sub>\<sigma> \<sigma>'" by (simp add: static_eval_state_to_state_let_prim)
   next
     case (Let_Fst \<rho> x\<^sub>p x\<^sub>1 x\<^sub>2 \<rho>\<^sub>p \<omega> x e \<kappa>)
     assume "\<sigma> = \<langle>LET x = FST x\<^sub>p in e;\<rho>;\<kappa>\<rangle>"
     and "\<sigma>' = \<langle>e;\<rho> ++ [x \<mapsto> \<omega>];\<kappa>\<rangle>"
     and "\<rho> x\<^sub>p = Some \<lbrace>prim.Pair x\<^sub>1 x\<^sub>2, \<rho>\<^sub>p\<rbrace>" and "\<rho>\<^sub>p x\<^sub>1 = Some \<omega>"
     with `(\<V>, \<C>) \<Turnstile>\<^sub>\<sigma> \<sigma>`
-    show "(\<V>, \<C>) \<Turnstile>\<^sub>\<sigma> \<sigma>'" by (simp add: accept_state_to_state_let_fst)
+    show "(\<V>, \<C>) \<Turnstile>\<^sub>\<sigma> \<sigma>'" by (simp add: static_eval_state_to_state_let_fst)
   next
     case (Let_Snd \<rho> x\<^sub>p x\<^sub>1 x\<^sub>2 \<rho>\<^sub>p \<omega> x e \<kappa>)
     assume "\<sigma> = \<langle>LET x = SND x\<^sub>p in e;\<rho>;\<kappa>\<rangle>"
     and "\<sigma>' = \<langle>e;\<rho> ++ [x \<mapsto> \<omega>];\<kappa>\<rangle>"
     and "\<rho> x\<^sub>p = Some \<lbrace>prim.Pair x\<^sub>1 x\<^sub>2, \<rho>\<^sub>p\<rbrace>" and "\<rho>\<^sub>p x\<^sub>2 = Some \<omega>"
     with `(\<V>, \<C>) \<Turnstile>\<^sub>\<sigma> \<sigma>`
-    show "(\<V>, \<C>) \<Turnstile>\<^sub>\<sigma> \<sigma>'" by (simp add: accept_state_to_state_let_snd)
+    show "(\<V>, \<C>) \<Turnstile>\<^sub>\<sigma> \<sigma>'" by (simp add: static_eval_state_to_state_let_snd)
   next
     case (Let_Case_Left \<rho> x\<^sub>s x\<^sub>l' \<rho>\<^sub>l \<omega>\<^sub>l x x\<^sub>l e\<^sub>l x\<^sub>r e\<^sub>r e \<kappa>)
 
@@ -868,7 +868,7 @@ proof -
     and "\<sigma>' = \<langle>e\<^sub>l;\<rho> ++ [x\<^sub>l \<mapsto> \<omega>\<^sub>l];\<langle>x,e,\<rho>\<rangle> # \<kappa>\<rangle>"
     and "\<rho> x\<^sub>s = Some \<lbrace>prim.Left x\<^sub>l', \<rho>\<^sub>l\<rbrace>" and "\<rho>\<^sub>l x\<^sub>l' = Some \<omega>\<^sub>l"
     with `(\<V>, \<C>) \<Turnstile>\<^sub>\<sigma> \<sigma>`
-    show "(\<V>, \<C>) \<Turnstile>\<^sub>\<sigma> \<sigma>'" by (simp add: accept_state_to_state_let_case_left)
+    show "(\<V>, \<C>) \<Turnstile>\<^sub>\<sigma> \<sigma>'" by (simp add: static_eval_state_to_state_let_case_left)
   next
     case (Let_Case_Right \<rho> x\<^sub>s x\<^sub>r' \<rho>\<^sub>r \<omega>\<^sub>r x x\<^sub>l e\<^sub>l x\<^sub>r e\<^sub>r e \<kappa>)
     assume "\<sigma> = \<langle>LET x = CASE x\<^sub>s LEFT x\<^sub>l |> e\<^sub>l RIGHT x\<^sub>r |> e\<^sub>r in e;\<rho>;\<kappa>\<rangle>"
@@ -876,7 +876,7 @@ proof -
     and "\<rho> x\<^sub>s = Some \<lbrace>prim.Right x\<^sub>r', \<rho>\<^sub>r\<rbrace>"
     and "\<rho>\<^sub>r x\<^sub>r' = Some \<omega>\<^sub>r"
     with `(\<V>, \<C>) \<Turnstile>\<^sub>\<sigma> \<sigma>`
-    show "(\<V>, \<C>) \<Turnstile>\<^sub>\<sigma> \<sigma>'" by (simp add: accept_state_to_state_let_case_right)
+    show "(\<V>, \<C>) \<Turnstile>\<^sub>\<sigma> \<sigma>'" by (simp add: static_eval_state_to_state_let_case_right)
   next
     case (Let_App \<rho> f f\<^sub>l x\<^sub>l e\<^sub>l \<rho>\<^sub>l x\<^sub>a \<omega>\<^sub>a x e \<kappa>)
     assume "\<sigma> = \<langle>LET x = APP f x\<^sub>a in e;\<rho>;\<kappa>\<rangle>"
@@ -884,12 +884,12 @@ proof -
     and "\<rho> f = Some \<lbrace>Abs f\<^sub>l x\<^sub>l e\<^sub>l, \<rho>\<^sub>l\<rbrace>"
     and "\<rho> x\<^sub>a = Some \<omega>\<^sub>a"
     with `(\<V>, \<C>) \<Turnstile>\<^sub>\<sigma> \<sigma>`
-    show "(\<V>, \<C>) \<Turnstile>\<^sub>\<sigma> \<sigma>'" by (simp add: accept_state_to_state_let_app)
+    show "(\<V>, \<C>) \<Turnstile>\<^sub>\<sigma> \<sigma>'" by (simp add: static_eval_state_to_state_let_app)
   qed
 
 qed
 
-lemma accept_preserved_under_seq_step_down: "
+lemma static_eval_preserved_under_seq_step_down: "
   (\<V>, \<C>) \<Turnstile>\<^sub>\<E> \<E> \<Longrightarrow> leaf \<E> \<pi> \<Longrightarrow> \<E> \<pi> = Some (\<langle>RESULT x; \<rho>; \<langle>x\<^sub>\<kappa>, e\<^sub>\<kappa>, \<rho>\<^sub>\<kappa>\<rangle> # \<kappa>\<rangle>) \<Longrightarrow> 
   \<langle>RESULT x; \<rho>; \<langle>x\<^sub>\<kappa>, e\<^sub>\<kappa>, \<rho>\<^sub>\<kappa>\<rangle> # \<kappa>\<rangle> \<hookrightarrow> \<sigma>' \<Longrightarrow> (\<V>, \<C>) \<Turnstile>\<^sub>\<E> \<E>(\<pi> ;; \<downharpoonleft>x\<^sub>\<kappa> \<mapsto> \<sigma>')
 "
@@ -899,7 +899,7 @@ proof
   have "(\<V>, \<C>) \<Turnstile>\<^sub>\<sigma> \<langle>RESULT x; \<rho>; \<langle>x\<^sub>\<kappa>, e\<^sub>\<kappa>, \<rho>\<^sub>\<kappa>\<rangle> # \<kappa>\<rangle>" by (simp add: static_eval_pool.simps)
   
   assume "\<langle>RESULT x; \<rho>; \<langle>x\<^sub>\<kappa>, e\<^sub>\<kappa>, \<rho>\<^sub>\<kappa>\<rangle> # \<kappa>\<rangle> \<hookrightarrow> \<sigma>'" with `(\<V>, \<C>) \<Turnstile>\<^sub>\<sigma> \<langle>RESULT x; \<rho>; \<langle>x\<^sub>\<kappa>, e\<^sub>\<kappa>, \<rho>\<^sub>\<kappa>\<rangle> # \<kappa>\<rangle>`
-  have "(\<V>, \<C>) \<Turnstile>\<^sub>\<sigma> \<sigma>'" by (simp add: accept_state_preserved_under_step)
+  have "(\<V>, \<C>) \<Turnstile>\<^sub>\<sigma> \<sigma>'" by (simp add: static_eval_state_preserved_under_step)
 
   from \<open>(\<V>, \<C>) \<Turnstile>\<^sub>\<E> \<E>\<close> \<open>(\<V>, \<C>) \<Turnstile>\<^sub>\<sigma> \<sigma>'\<close>
   show "\<forall>\<pi>' \<sigma>. (\<E>(\<pi> ;; \<downharpoonleft>x\<^sub>\<kappa> \<mapsto> \<sigma>')) \<pi>' = Some \<sigma> \<longrightarrow> (\<V>, \<C>) \<Turnstile>\<^sub>\<sigma> \<sigma>" by (simp add: static_eval_pool.simps)
@@ -907,7 +907,7 @@ proof
 qed
 
 
-lemma accept_preserved_under_seq_step_up: "
+lemma static_eval_preserved_under_seq_step_up: "
   (\<V>, \<C>) \<Turnstile>\<^sub>\<E> \<E> \<Longrightarrow> leaf \<E> \<pi> \<Longrightarrow> \<E> \<pi> = Some (\<langle>LET x = b in e; \<rho>; \<kappa>\<rangle>) \<Longrightarrow> 
   \<langle>LET x = b in e; \<rho>; \<kappa>\<rangle> \<hookrightarrow> \<sigma>' \<Longrightarrow> (\<V>, \<C>) \<Turnstile>\<^sub>\<E> \<E>(\<pi>;;\<upharpoonleft>x \<mapsto> \<sigma>')
 "
@@ -916,14 +916,14 @@ proof
   have "(\<V>, \<C>) \<Turnstile>\<^sub>\<sigma> \<langle>LET x = b in e; \<rho>; \<kappa>\<rangle>" by (simp add: static_eval_pool.simps)
 
   assume "\<langle>LET x = b in e; \<rho>; \<kappa>\<rangle> \<hookrightarrow> \<sigma>'" with `(\<V>, \<C>) \<Turnstile>\<^sub>\<sigma> \<langle>LET x = b in e; \<rho>; \<kappa>\<rangle>`
-  have "(\<V>, \<C>) \<Turnstile>\<^sub>\<sigma> \<sigma>'" by (simp add: accept_state_preserved_under_step)
+  have "(\<V>, \<C>) \<Turnstile>\<^sub>\<sigma> \<sigma>'" by (simp add: static_eval_state_preserved_under_step)
 
   from \<open>(\<V>, \<C>) \<Turnstile>\<^sub>\<E> \<E>\<close> \<open>(\<V>, \<C>) \<Turnstile>\<^sub>\<sigma> \<sigma>'\<close>
   show "\<forall>\<pi>' \<sigma>. (\<E>(\<pi> ;; \<upharpoonleft>x \<mapsto> \<sigma>')) \<pi>' = Some \<sigma> \<longrightarrow> (\<V>, \<C>) \<Turnstile>\<^sub>\<sigma> \<sigma>" by (simp add: static_eval_pool.simps)
 qed
 
 
-lemma accept_preserved_under_seq_step: "
+lemma static_eval_preserved_under_seq_step: "
   (\<V>, \<C>) \<Turnstile>\<^sub>\<E> \<E> \<Longrightarrow> leaf \<E> \<pi> \<Longrightarrow> \<E> \<pi> = Some (\<langle>LET x = b in e; \<rho>; \<kappa>\<rangle>) \<Longrightarrow> 
   \<langle>LET x = b in e; \<rho>; \<kappa>\<rangle> \<hookrightarrow> \<sigma>' \<Longrightarrow> (\<V>, \<C>) \<Turnstile>\<^sub>\<E> \<E>(\<pi> ;; `x \<mapsto> \<sigma>')
 "
@@ -932,13 +932,13 @@ proof
   have "(\<V>, \<C>) \<Turnstile>\<^sub>\<sigma> \<langle>LET x = b in e; \<rho>; \<kappa>\<rangle>" by (simp add: static_eval_pool.simps)
 
   assume "\<langle>LET x = b in e; \<rho>; \<kappa>\<rangle> \<hookrightarrow> \<sigma>'" with `(\<V>, \<C>) \<Turnstile>\<^sub>\<sigma> \<langle>LET x = b in e; \<rho>; \<kappa>\<rangle>`
-  have "(\<V>, \<C>) \<Turnstile>\<^sub>\<sigma> \<sigma>'" by (simp add: accept_state_preserved_under_step)
+  have "(\<V>, \<C>) \<Turnstile>\<^sub>\<sigma> \<sigma>'" by (simp add: static_eval_state_preserved_under_step)
 
   from \<open>(\<V>, \<C>) \<Turnstile>\<^sub>\<E> \<E>\<close> \<open>(\<V>, \<C>) \<Turnstile>\<^sub>\<sigma> \<sigma>'\<close>
   show "\<forall>\<pi>' \<sigma>. (\<E>(\<pi> ;; `x \<mapsto> \<sigma>')) \<pi>' = Some \<sigma> \<longrightarrow> (\<V>, \<C>) \<Turnstile>\<^sub>\<sigma> \<sigma>" by (simp add: static_eval_pool.simps)
 qed
 
-lemma accept_pool_to_exp_let: "
+lemma static_eval_pool_to_exp_let: "
   (\<V>, \<C>) \<Turnstile>\<^sub>\<E> \<E> \<Longrightarrow>
   \<E> \<pi> = Some (\<langle>LET x = b in e; \<rho>; \<kappa>\<rangle>) \<Longrightarrow>
   (\<V>, \<C>) \<Turnstile>\<^sub>e e
@@ -946,11 +946,11 @@ lemma accept_pool_to_exp_let: "
 proof -
  assume "(\<V>, \<C>) \<Turnstile>\<^sub>\<E> \<E>" and "\<E> \<pi> = Some (\<langle>LET x = b in e; \<rho>; \<kappa>\<rangle>)" then
  have "(\<V>, \<C>) \<Turnstile>\<^sub>\<sigma> \<langle>LET x = b in e; \<rho>; \<kappa>\<rangle>" by (simp add: static_eval_pool.simps) then
- show "(\<V>, \<C>) \<Turnstile>\<^sub>e e " by (blast intro: accept_state_to_exp_let)
+ show "(\<V>, \<C>) \<Turnstile>\<^sub>e e " by (blast intro: static_eval_state_to_exp_let)
 qed
 
 
-lemma accept_pool_let_sync_send_values_relate: "
+lemma static_eval_pool_let_sync_send_values_relate: "
   (\<V>, \<C>) \<Turnstile>\<^sub>\<E> \<E> \<Longrightarrow>
   \<E> \<pi>\<^sub>s = Some (\<langle>LET x\<^sub>s = SYNC x\<^sub>s\<^sub>e in e\<^sub>s; \<rho>\<^sub>s; \<kappa>\<^sub>s\<rangle>) \<Longrightarrow>
   \<rho>\<^sub>s x\<^sub>s\<^sub>e = Some \<lbrace>Send_Evt x\<^sub>s\<^sub>c x\<^sub>m, \<rho>\<^sub>s\<^sub>e\<rbrace> \<Longrightarrow>
@@ -965,7 +965,7 @@ proof -
 
   from `(\<V>, \<C>) \<Turnstile>\<^sub>\<E> \<E>` and `\<E> \<pi>\<^sub>s = Some (\<langle>LET x\<^sub>s = SYNC x\<^sub>s\<^sub>e in e\<^sub>s; \<rho>\<^sub>s; \<kappa>\<^sub>s\<rangle>)`
   have "(\<V>, \<C>) \<Turnstile>\<^sub>\<sigma> \<langle>LET x\<^sub>s = SYNC x\<^sub>s\<^sub>e in e\<^sub>s; \<rho>\<^sub>s; \<kappa>\<^sub>s\<rangle>" by (simp add: static_eval_pool.simps) then
-  have "(\<V>, \<C>) \<Turnstile>\<^sub>e LET x\<^sub>s = SYNC x\<^sub>s\<^sub>e in e\<^sub>s" "(\<V>, \<C>) \<Turnstile>\<^sub>\<rho> \<rho>\<^sub>s" by (simp add: accept_state.simps)+
+  have "(\<V>, \<C>) \<Turnstile>\<^sub>e LET x\<^sub>s = SYNC x\<^sub>s\<^sub>e in e\<^sub>s" "(\<V>, \<C>) \<Turnstile>\<^sub>\<rho> \<rho>\<^sub>s" by (simp add: static_eval_state.simps)+
 
   from `(\<V>, \<C>) \<Turnstile>\<^sub>\<rho> \<rho>\<^sub>s` and `\<rho>\<^sub>s x\<^sub>s\<^sub>e = Some \<lbrace>Send_Evt x\<^sub>s\<^sub>c x\<^sub>m, \<rho>\<^sub>s\<^sub>e\<rbrace>`
   have "{|\<lbrace>Send_Evt x\<^sub>s\<^sub>c x\<^sub>m, \<rho>\<^sub>s\<^sub>e\<rbrace>|} \<subseteq> \<V> x\<^sub>s\<^sub>e" and "(\<V>, \<C>) \<Turnstile>\<^sub>\<omega> \<lbrace>Send_Evt x\<^sub>s\<^sub>c x\<^sub>m, \<rho>\<^sub>s\<^sub>e\<rbrace>" by (blast intro: static_eval_env.cases)+
@@ -991,7 +991,7 @@ proof -
 
 qed
 
-lemma accept_pool_let_sync_send_message_relate: "
+lemma static_eval_pool_let_sync_send_message_relate: "
   (\<V>, \<C>) \<Turnstile>\<^sub>\<E> \<E> \<Longrightarrow>
   \<E> \<pi>\<^sub>s = Some (\<langle>LET x\<^sub>s = SYNC x\<^sub>s\<^sub>e in e\<^sub>s; \<rho>\<^sub>s; \<kappa>\<^sub>s\<rangle>) \<Longrightarrow>
   \<rho>\<^sub>s x\<^sub>s\<^sub>e = Some \<lbrace>Send_Evt x\<^sub>s\<^sub>c x\<^sub>m, \<rho>\<^sub>s\<^sub>e\<rbrace> \<Longrightarrow>
@@ -1006,7 +1006,7 @@ proof -
 
   from `(\<V>, \<C>) \<Turnstile>\<^sub>\<E> \<E>` and `\<E> \<pi>\<^sub>s = Some (\<langle>LET x\<^sub>s = SYNC x\<^sub>s\<^sub>e in e\<^sub>s; \<rho>\<^sub>s; \<kappa>\<^sub>s\<rangle>)`
   have "(\<V>, \<C>) \<Turnstile>\<^sub>\<sigma> \<langle>LET x\<^sub>s = SYNC x\<^sub>s\<^sub>e in e\<^sub>s; \<rho>\<^sub>s; \<kappa>\<^sub>s\<rangle>" by (simp add: static_eval_pool.simps) then
-  have "(\<V>, \<C>) \<Turnstile>\<^sub>\<rho> \<rho>\<^sub>s" by (simp add: accept_state.simps)
+  have "(\<V>, \<C>) \<Turnstile>\<^sub>\<rho> \<rho>\<^sub>s" by (simp add: static_eval_state.simps)
   with `\<rho>\<^sub>s x\<^sub>s\<^sub>e = Some \<lbrace>Send_Evt x\<^sub>s\<^sub>c x\<^sub>m, \<rho>\<^sub>s\<^sub>e\<rbrace>`
   have "(\<V>, \<C>) \<Turnstile>\<^sub>\<omega> \<lbrace>Send_Evt x\<^sub>s\<^sub>c x\<^sub>m, \<rho>\<^sub>s\<^sub>e\<rbrace>" by (blast intro: static_eval_env.cases) then
   have "(\<V>, \<C>) \<Turnstile>\<^sub>\<rho> \<rho>\<^sub>s\<^sub>e" by (blast intro: static_eval_value.cases)
@@ -1014,7 +1014,7 @@ proof -
   show "{|\<omega>\<^sub>m|} \<subseteq> \<V> x\<^sub>m \<and> (\<V>, \<C>) \<Turnstile>\<^sub>\<omega> \<omega>\<^sub>m" by (blast intro: static_eval_env.cases)
 qed
 
-lemma accept_pool_to_env_let_sync_send: "
+lemma static_eval_pool_to_env_let_sync_send: "
   (\<V>, \<C>) \<Turnstile>\<^sub>\<E> \<E> \<Longrightarrow>
   \<E> \<pi>\<^sub>s = Some (\<langle>LET x\<^sub>s = SYNC x\<^sub>s\<^sub>e in e\<^sub>s; \<rho>\<^sub>s; \<kappa>\<^sub>s\<rangle>) \<Longrightarrow>
   \<rho>\<^sub>s x\<^sub>s\<^sub>e = Some \<lbrace>Send_Evt x\<^sub>s\<^sub>c x\<^sub>m, \<rho>\<^sub>s\<^sub>e\<rbrace> \<Longrightarrow>
@@ -1029,7 +1029,7 @@ proof
 
   from `(\<V>, \<C>) \<Turnstile>\<^sub>\<E> \<E>` and `\<E> \<pi>\<^sub>s = Some (\<langle>LET x\<^sub>s = SYNC x\<^sub>s\<^sub>e in e\<^sub>s; \<rho>\<^sub>s; \<kappa>\<^sub>s\<rangle>)`
   have "(\<V>, \<C>) \<Turnstile>\<^sub>\<sigma> \<langle>LET x\<^sub>s = SYNC x\<^sub>s\<^sub>e in e\<^sub>s; \<rho>\<^sub>s; \<kappa>\<^sub>s\<rangle>" by (simp add: static_eval_pool.simps) then
-  have "(\<V>, \<C>) \<Turnstile>\<^sub>\<rho> \<rho>\<^sub>s" by (simp add: accept_state.simps)+
+  have "(\<V>, \<C>) \<Turnstile>\<^sub>\<rho> \<rho>\<^sub>s" by (simp add: static_eval_state.simps)+
 
   have "{^\<lparr>\<rparr>} \<subseteq> \<V> x\<^sub>s"
   proof (cases c)
@@ -1039,7 +1039,7 @@ proof
     and  `(\<V>, \<C>) \<Turnstile>\<^sub>\<E> \<E>`
     and `\<E> \<pi>\<^sub>s = Some (\<langle>LET x\<^sub>s = SYNC x\<^sub>s\<^sub>e in e\<^sub>s; \<rho>\<^sub>s; \<kappa>\<^sub>s\<rangle>)`
     and `\<rho>\<^sub>s x\<^sub>s\<^sub>e = Some \<lbrace>Send_Evt x\<^sub>s\<^sub>c x\<^sub>m, \<rho>\<^sub>s\<^sub>e\<rbrace>`
-    show "{^\<lparr>\<rparr>} \<subseteq> \<V> x\<^sub>s" using accept_pool_let_sync_send_values_relate by simp
+    show "{^\<lparr>\<rparr>} \<subseteq> \<V> x\<^sub>s" using static_eval_pool_let_sync_send_values_relate by simp
   qed
   
   have "(\<V>, \<C>) \<Turnstile>\<^sub>\<omega> \<lbrace>\<rbrace>" by (simp add: Unit)
@@ -1055,7 +1055,7 @@ proof
 qed
 
 
-lemma accept_pool_let_sync_recv_values_relate: "
+lemma static_eval_pool_let_sync_recv_values_relate: "
   (\<V>, \<C>) \<Turnstile>\<^sub>\<E> \<E> \<Longrightarrow>
   \<E> \<pi>\<^sub>r = Some (\<langle>LET x\<^sub>r = SYNC x\<^sub>r\<^sub>e in e\<^sub>r; \<rho>\<^sub>r; \<kappa>\<^sub>r\<rangle>) \<Longrightarrow>
   \<rho>\<^sub>r x\<^sub>r\<^sub>e = Some \<lbrace>Recv_Evt x\<^sub>r\<^sub>c, \<rho>\<^sub>r\<^sub>e\<rbrace> \<Longrightarrow>
@@ -1070,7 +1070,7 @@ proof -
 
   from `(\<V>, \<C>) \<Turnstile>\<^sub>\<E> \<E>` and `\<E> \<pi>\<^sub>r = Some (\<langle>LET x\<^sub>r = SYNC x\<^sub>r\<^sub>e in e\<^sub>r; \<rho>\<^sub>r; \<kappa>\<^sub>r\<rangle>)`
   have "(\<V>, \<C>) \<Turnstile>\<^sub>\<sigma> \<langle>LET x\<^sub>r = SYNC x\<^sub>r\<^sub>e in e\<^sub>r; \<rho>\<^sub>r; \<kappa>\<^sub>r\<rangle>" by (simp add: static_eval_pool.simps) then
-  have "(\<V>, \<C>) \<Turnstile>\<^sub>e LET x\<^sub>r = SYNC x\<^sub>r\<^sub>e in e\<^sub>r" "(\<V>, \<C>) \<Turnstile>\<^sub>\<rho> \<rho>\<^sub>r" by (simp add: accept_state.simps)+
+  have "(\<V>, \<C>) \<Turnstile>\<^sub>e LET x\<^sub>r = SYNC x\<^sub>r\<^sub>e in e\<^sub>r" "(\<V>, \<C>) \<Turnstile>\<^sub>\<rho> \<rho>\<^sub>r" by (simp add: static_eval_state.simps)+
 
   from `(\<V>, \<C>) \<Turnstile>\<^sub>\<rho> \<rho>\<^sub>r` and `\<rho>\<^sub>r x\<^sub>r\<^sub>e = Some \<lbrace>Recv_Evt x\<^sub>r\<^sub>c, \<rho>\<^sub>r\<^sub>e\<rbrace>`
   have "{|\<lbrace>Recv_Evt x\<^sub>r\<^sub>c, \<rho>\<^sub>r\<^sub>e\<rbrace>|} \<subseteq> \<V> x\<^sub>r\<^sub>e" and "(\<V>, \<C>) \<Turnstile>\<^sub>\<omega> \<lbrace>Recv_Evt x\<^sub>r\<^sub>c, \<rho>\<^sub>r\<^sub>e\<rbrace>" by (blast intro: static_eval_env.cases)+
@@ -1096,7 +1096,7 @@ proof -
 qed
 
 
-lemma accept_pool_to_stack_let: "
+lemma static_eval_pool_to_stack_let: "
   (\<V>, \<C>) \<Turnstile>\<^sub>\<E> \<E> \<Longrightarrow>
   \<E> \<pi> = Some (\<langle>LET x = b in e; \<rho>; \<kappa>\<rangle>) \<Longrightarrow>
   (\<V>, \<C>) \<Turnstile>\<^sub>\<kappa> \<V> (\<lfloor>e\<rfloor>) \<Rrightarrow> \<kappa>
@@ -1104,10 +1104,10 @@ lemma accept_pool_to_stack_let: "
 proof -
   assume "(\<V>, \<C>) \<Turnstile>\<^sub>\<E> \<E>" and "\<E> \<pi> = Some (\<langle>LET x = b in e; \<rho>; \<kappa>\<rangle>)" then
   have "(\<V>, \<C>) \<Turnstile>\<^sub>\<sigma> \<langle>LET x = b in e; \<rho>; \<kappa>\<rangle>" by (simp add: static_eval_pool.simps) then
-  show "(\<V>, \<C>) \<Turnstile>\<^sub>\<kappa> \<V> (\<lfloor>e\<rfloor>) \<Rrightarrow> \<kappa>" by (simp add: accept_state_to_stack_let)
+  show "(\<V>, \<C>) \<Turnstile>\<^sub>\<kappa> \<V> (\<lfloor>e\<rfloor>) \<Rrightarrow> \<kappa>" by (simp add: static_eval_state_to_stack_let)
 qed
 
-lemma accept_pool_to_env_let_sync_recv: "
+lemma static_eval_pool_to_env_let_sync_recv: "
   (\<V>, \<C>) \<Turnstile>\<^sub>\<E> \<E> \<Longrightarrow>
   \<E> \<pi>\<^sub>s = Some (\<langle>LET x\<^sub>s = SYNC x\<^sub>s\<^sub>e in e\<^sub>s; \<rho>\<^sub>s; \<kappa>\<^sub>s\<rangle>) \<Longrightarrow>
   \<rho>\<^sub>s x\<^sub>s\<^sub>e = Some \<lbrace>Send_Evt x\<^sub>s\<^sub>c x\<^sub>m, \<rho>\<^sub>s\<^sub>e\<rbrace> \<Longrightarrow>
@@ -1123,7 +1123,7 @@ proof
   and "\<E> \<pi>\<^sub>s = Some (\<langle>LET x\<^sub>s = SYNC x\<^sub>s\<^sub>e in e\<^sub>s; \<rho>\<^sub>s; \<kappa>\<^sub>s\<rangle>)"
   and "\<rho>\<^sub>s x\<^sub>s\<^sub>e = Some \<lbrace>Send_Evt x\<^sub>s\<^sub>c x\<^sub>m, \<rho>\<^sub>s\<^sub>e\<rbrace>"
   and "\<rho>\<^sub>s\<^sub>e x\<^sub>m = Some \<omega>\<^sub>m" then
-  have "{|\<omega>\<^sub>m|} \<subseteq> \<V> x\<^sub>m" "(\<V>, \<C>) \<Turnstile>\<^sub>\<omega> \<omega>\<^sub>m" using accept_pool_let_sync_send_message_relate by auto
+  have "{|\<omega>\<^sub>m|} \<subseteq> \<V> x\<^sub>m" "(\<V>, \<C>) \<Turnstile>\<^sub>\<omega> \<omega>\<^sub>m" using static_eval_pool_let_sync_send_message_relate by auto
 
   assume "\<rho>\<^sub>s\<^sub>e x\<^sub>s\<^sub>c = Some \<lbrace>c\<rbrace>"
   and "\<E> \<pi>\<^sub>r = Some (\<langle>LET x\<^sub>r = SYNC x\<^sub>r\<^sub>e in e\<^sub>r; \<rho>\<^sub>r; \<kappa>\<^sub>r\<rangle>)"
@@ -1132,7 +1132,7 @@ proof
 
   from `(\<V>, \<C>) \<Turnstile>\<^sub>\<E> \<E>` and `\<E> \<pi>\<^sub>r = Some (\<langle>LET x\<^sub>r = SYNC x\<^sub>r\<^sub>e in e\<^sub>r; \<rho>\<^sub>r; \<kappa>\<^sub>r\<rangle>)`
   have "(\<V>, \<C>) \<Turnstile>\<^sub>\<sigma> \<langle>LET x\<^sub>r = SYNC x\<^sub>r\<^sub>e in e\<^sub>r; \<rho>\<^sub>r; \<kappa>\<^sub>r\<rangle>" by (simp add: static_eval_pool.simps) then
-  have "(\<V>, \<C>) \<Turnstile>\<^sub>\<rho> \<rho>\<^sub>r" by (simp add: accept_state.simps)+
+  have "(\<V>, \<C>) \<Turnstile>\<^sub>\<rho> \<rho>\<^sub>r" by (simp add: static_eval_state.simps)+
 
 
   have "\<V> x\<^sub>m \<subseteq> \<V> x\<^sub>r"
@@ -1146,14 +1146,14 @@ proof
     and `\<rho>\<^sub>s x\<^sub>s\<^sub>e = Some \<lbrace>Send_Evt x\<^sub>s\<^sub>c x\<^sub>m, \<rho>\<^sub>s\<^sub>e\<rbrace>`
     and `\<E> \<pi>\<^sub>s = Some (\<langle>LET x\<^sub>s = SYNC x\<^sub>s\<^sub>e in e\<^sub>s; \<rho>\<^sub>s; \<kappa>\<^sub>s\<rangle>)`
     and `\<rho>\<^sub>s\<^sub>e x\<^sub>m = Some \<omega>\<^sub>m`
-    have "\<V> x\<^sub>m \<subseteq> \<C> x\<^sub>c" using \<open>\<rho>\<^sub>s\<^sub>e x\<^sub>s\<^sub>c = Some \<lbrace>c\<rbrace>\<close> accept_pool_let_sync_send_values_relate by blast
+    have "\<V> x\<^sub>m \<subseteq> \<C> x\<^sub>c" using \<open>\<rho>\<^sub>s\<^sub>e x\<^sub>s\<^sub>c = Some \<lbrace>c\<rbrace>\<close> static_eval_pool_let_sync_send_values_relate by blast
 
     with `c = Ch \<pi>\<^sub>c x\<^sub>c`
     and `\<rho>\<^sub>r\<^sub>e x\<^sub>r\<^sub>c = Some \<lbrace>c\<rbrace>`
     and `(\<V>, \<C>) \<Turnstile>\<^sub>\<E> \<E>`
     and `\<E> \<pi>\<^sub>r = Some (\<langle>LET x\<^sub>r = SYNC x\<^sub>r\<^sub>e in e\<^sub>r; \<rho>\<^sub>r; \<kappa>\<^sub>r\<rangle>)`
     and `\<rho>\<^sub>r x\<^sub>r\<^sub>e = Some \<lbrace>Recv_Evt x\<^sub>r\<^sub>c, \<rho>\<^sub>r\<^sub>e\<rbrace>`
-    have "\<C> x\<^sub>c \<subseteq> \<V> x\<^sub>r" using  accept_pool_let_sync_recv_values_relate by auto
+    have "\<C> x\<^sub>c \<subseteq> \<V> x\<^sub>r" using  static_eval_pool_let_sync_recv_values_relate by auto
 
     from `\<V> x\<^sub>m \<subseteq> \<C> x\<^sub>c` and `\<C> x\<^sub>c \<subseteq> \<V> x\<^sub>r`
     show "\<V> x\<^sub>m \<subseteq> \<V> x\<^sub>r" by simp
@@ -1164,7 +1164,7 @@ proof
 
   from `(\<V>, \<C>) \<Turnstile>\<^sub>\<E> \<E>` and `\<E> \<pi>\<^sub>s = Some (\<langle>LET x\<^sub>s = SYNC x\<^sub>s\<^sub>e in e\<^sub>s; \<rho>\<^sub>s; \<kappa>\<^sub>s\<rangle>)`
   have "(\<V>, \<C>) \<Turnstile>\<^sub>\<sigma> \<langle>LET x\<^sub>s = SYNC x\<^sub>s\<^sub>e in e\<^sub>s; \<rho>\<^sub>s; \<kappa>\<^sub>s\<rangle>" by (simp add: static_eval_pool.simps) then
-  have "(\<V>, \<C>) \<Turnstile>\<^sub>\<rho> \<rho>\<^sub>s" by (simp add: accept_state.simps)+
+  have "(\<V>, \<C>) \<Turnstile>\<^sub>\<rho> \<rho>\<^sub>s" by (simp add: static_eval_state.simps)+
   {
     fix x' \<omega>'
     assume "(\<rho>\<^sub>r(x\<^sub>r \<mapsto> \<omega>\<^sub>m)) x' = Some \<omega>'" "x' \<noteq> x\<^sub>r" then
@@ -1177,7 +1177,7 @@ proof
 qed
 
 
-lemma accept_preserved_under_sync: "
+lemma static_eval_preserved_under_sync: "
   (\<V>, \<C>) \<Turnstile>\<^sub>\<E> \<E> \<Longrightarrow>
   \<E> \<pi>\<^sub>s = Some (\<langle>LET x\<^sub>s = SYNC x\<^sub>s\<^sub>e in e\<^sub>s; \<rho>\<^sub>s; \<kappa>\<^sub>s\<rangle>) \<Longrightarrow>
   \<rho>\<^sub>s x\<^sub>s\<^sub>e = Some \<lbrace>Send_Evt x\<^sub>s\<^sub>c x\<^sub>m, \<rho>\<^sub>s\<^sub>e\<rbrace> \<Longrightarrow>
@@ -1200,20 +1200,20 @@ proof
 
 
   from \<open>(\<V>, \<C>) \<Turnstile>\<^sub>\<E> \<E>\<close> and \<open>\<E> \<pi>\<^sub>s = Some (\<langle>LET x\<^sub>s = SYNC x\<^sub>s\<^sub>e in e\<^sub>s;\<rho>\<^sub>s;\<kappa>\<^sub>s\<rangle>)\<close> 
-  have "(\<V>, \<C>) \<Turnstile>\<^sub>e e\<^sub>s" by (blast intro: accept_pool_to_exp_let)
+  have "(\<V>, \<C>) \<Turnstile>\<^sub>e e\<^sub>s" by (blast intro: static_eval_pool_to_exp_let)
 
   from \<open>(\<V>, \<C>) \<Turnstile>\<^sub>\<E> \<E>\<close> \<open>\<E> \<pi>\<^sub>s = Some (\<langle>LET x\<^sub>s = SYNC x\<^sub>s\<^sub>e in e\<^sub>s;\<rho>\<^sub>s;\<kappa>\<^sub>s\<rangle>)\<close> 
   and \<open>\<rho>\<^sub>s x\<^sub>s\<^sub>e = Some \<lbrace>Send_Evt x\<^sub>s\<^sub>c x\<^sub>m, \<rho>\<^sub>s\<^sub>e\<rbrace>\<close> \<open>\<rho>\<^sub>s\<^sub>e x\<^sub>s\<^sub>c = Some \<lbrace>c\<rbrace>\<close> 
-  have "(\<V>, \<C>) \<Turnstile>\<^sub>\<rho> \<rho>\<^sub>s(x\<^sub>s \<mapsto> \<lbrace>\<rbrace>)" by (blast intro: accept_pool_to_env_let_sync_send)
+  have "(\<V>, \<C>) \<Turnstile>\<^sub>\<rho> \<rho>\<^sub>s(x\<^sub>s \<mapsto> \<lbrace>\<rbrace>)" by (blast intro: static_eval_pool_to_env_let_sync_send)
 
   from \<open>(\<V>, \<C>) \<Turnstile>\<^sub>\<E> \<E>\<close> and \<open>\<E> \<pi>\<^sub>s = Some (\<langle>LET x\<^sub>s = SYNC x\<^sub>s\<^sub>e in e\<^sub>s;\<rho>\<^sub>s;\<kappa>\<^sub>s\<rangle>)\<close>
-  have  "(\<V>, \<C>) \<Turnstile>\<^sub>\<kappa> \<V> (\<lfloor>e\<^sub>s\<rfloor>) \<Rrightarrow> \<kappa>\<^sub>s" by (blast intro: accept_pool_to_stack_let)
+  have  "(\<V>, \<C>) \<Turnstile>\<^sub>\<kappa> \<V> (\<lfloor>e\<^sub>s\<rfloor>) \<Rrightarrow> \<kappa>\<^sub>s" by (blast intro: static_eval_pool_to_stack_let)
 
   from `(\<V>, \<C>) \<Turnstile>\<^sub>e e\<^sub>s` and `(\<V>, \<C>) \<Turnstile>\<^sub>\<rho> \<rho>\<^sub>s(x\<^sub>s \<mapsto> \<lbrace>\<rbrace>)` and `(\<V>, \<C>) \<Turnstile>\<^sub>\<kappa> \<V> (\<lfloor>e\<^sub>s\<rfloor>) \<Rrightarrow> \<kappa>\<^sub>s`
-  have "(\<V>, \<C>) \<Turnstile>\<^sub>\<sigma> \<langle>e\<^sub>s;\<rho>\<^sub>s(x\<^sub>s \<mapsto> \<lbrace>\<rbrace>);\<kappa>\<^sub>s\<rangle>" by (blast intro: accept_state.intros)
+  have "(\<V>, \<C>) \<Turnstile>\<^sub>\<sigma> \<langle>e\<^sub>s;\<rho>\<^sub>s(x\<^sub>s \<mapsto> \<lbrace>\<rbrace>);\<kappa>\<^sub>s\<rangle>" by (blast intro: static_eval_state.intros)
 
   from \<open>(\<V>, \<C>) \<Turnstile>\<^sub>\<E> \<E>\<close> and \<open>\<E> \<pi>\<^sub>r = Some (\<langle>LET x\<^sub>r = SYNC x\<^sub>r\<^sub>e in e\<^sub>r;\<rho>\<^sub>r;\<kappa>\<^sub>r\<rangle>)\<close> 
-  have "(\<V>, \<C>) \<Turnstile>\<^sub>e e\<^sub>r" by (blast intro: accept_pool_to_exp_let)
+  have "(\<V>, \<C>) \<Turnstile>\<^sub>e e\<^sub>r" by (blast intro: static_eval_pool_to_exp_let)
 
   from \<open>(\<V>, \<C>) \<Turnstile>\<^sub>\<E> \<E>\<close> 
   and \<open>\<E> \<pi>\<^sub>s = Some (\<langle>LET x\<^sub>s = SYNC x\<^sub>s\<^sub>e in e\<^sub>s;\<rho>\<^sub>s;\<kappa>\<^sub>s\<rangle>)\<close> 
@@ -1221,13 +1221,13 @@ proof
   and \<open>\<rho>\<^sub>s\<^sub>e x\<^sub>m = Some \<omega>\<^sub>m\<close> \<open>\<rho>\<^sub>s\<^sub>e x\<^sub>s\<^sub>c = Some \<lbrace>c\<rbrace>\<close>
   and \<open>\<E> \<pi>\<^sub>r = Some (\<langle>LET x\<^sub>r = SYNC x\<^sub>r\<^sub>e in e\<^sub>r;\<rho>\<^sub>r;\<kappa>\<^sub>r\<rangle>)\<close> 
   and \<open>\<rho>\<^sub>r x\<^sub>r\<^sub>e = Some \<lbrace>Recv_Evt x\<^sub>r\<^sub>c, \<rho>\<^sub>r\<^sub>e\<rbrace>\<close> \<open>\<rho>\<^sub>r\<^sub>e x\<^sub>r\<^sub>c = Some \<lbrace>c\<rbrace>\<close> 
-  have "(\<V>, \<C>) \<Turnstile>\<^sub>\<rho> \<rho>\<^sub>r(x\<^sub>r \<mapsto> \<omega>\<^sub>m)" by (blast intro: accept_pool_to_env_let_sync_recv)
+  have "(\<V>, \<C>) \<Turnstile>\<^sub>\<rho> \<rho>\<^sub>r(x\<^sub>r \<mapsto> \<omega>\<^sub>m)" by (blast intro: static_eval_pool_to_env_let_sync_recv)
 
   from \<open>(\<V>, \<C>) \<Turnstile>\<^sub>\<E> \<E>\<close> and \<open>\<E> \<pi>\<^sub>r = Some (\<langle>LET x\<^sub>r = SYNC x\<^sub>r\<^sub>e in e\<^sub>r;\<rho>\<^sub>r;\<kappa>\<^sub>r\<rangle>)\<close>
-  have  "(\<V>, \<C>) \<Turnstile>\<^sub>\<kappa> \<V> (\<lfloor>e\<^sub>r\<rfloor>) \<Rrightarrow> \<kappa>\<^sub>r" by (blast intro: accept_pool_to_stack_let)
+  have  "(\<V>, \<C>) \<Turnstile>\<^sub>\<kappa> \<V> (\<lfloor>e\<^sub>r\<rfloor>) \<Rrightarrow> \<kappa>\<^sub>r" by (blast intro: static_eval_pool_to_stack_let)
 
   from `(\<V>, \<C>) \<Turnstile>\<^sub>e e\<^sub>r` and `(\<V>, \<C>) \<Turnstile>\<^sub>\<rho> \<rho>\<^sub>r(x\<^sub>r \<mapsto> \<omega>\<^sub>m)` and `(\<V>, \<C>) \<Turnstile>\<^sub>\<kappa> \<V> (\<lfloor>e\<^sub>r\<rfloor>) \<Rrightarrow> \<kappa>\<^sub>r`
-  have "(\<V>, \<C>) \<Turnstile>\<^sub>\<sigma> \<langle>e\<^sub>r;\<rho>\<^sub>r(x\<^sub>r \<mapsto> \<omega>\<^sub>m);\<kappa>\<^sub>r\<rangle>" by (blast intro: accept_state.intros)
+  have "(\<V>, \<C>) \<Turnstile>\<^sub>\<sigma> \<langle>e\<^sub>r;\<rho>\<^sub>r(x\<^sub>r \<mapsto> \<omega>\<^sub>m);\<kappa>\<^sub>r\<rangle>" by (blast intro: static_eval_state.intros)
 
   {
     fix \<pi> \<sigma>
@@ -1242,7 +1242,7 @@ proof
 qed
 
 
-lemma accept_pool_to_env_let_chan: "
+lemma static_eval_pool_to_env_let_chan: "
   (\<V>, \<C>) \<Turnstile>\<^sub>\<E> \<E> \<Longrightarrow>
   \<E> \<pi> = Some (\<langle>LET x = CHAN \<lparr>\<rparr> in e; \<rho>; \<kappa>\<rangle>) \<Longrightarrow> 
   (\<V>, \<C>) \<Turnstile>\<^sub>\<rho> \<rho>(x \<mapsto> \<lbrace>Ch \<pi> x\<rbrace>)
@@ -1250,12 +1250,12 @@ lemma accept_pool_to_env_let_chan: "
 proof
   assume "(\<V>, \<C>) \<Turnstile>\<^sub>\<E> \<E>" and "\<E> \<pi> = Some (\<langle>LET x = CHAN \<lparr>\<rparr> in e; \<rho>; \<kappa>\<rangle>)" then
   have "(\<V>, \<C>) \<Turnstile>\<^sub>\<sigma> \<langle>LET x = CHAN \<lparr>\<rparr> in e; \<rho>; \<kappa>\<rangle>" by (blast intro: static_eval_pool.cases) then
-  have "(\<V>, \<C>) \<Turnstile>\<^sub>e LET x = CHAN \<lparr>\<rparr> in e" by (blast intro: accept_state.cases) then
+  have "(\<V>, \<C>) \<Turnstile>\<^sub>e LET x = CHAN \<lparr>\<rparr> in e" by (blast intro: static_eval_state.cases) then
   have "{^Chan x} \<subseteq> \<V> x"  by (blast intro: static_eval.cases)
   have "(\<V>, \<C>) \<Turnstile>\<^sub>\<omega> \<lbrace>Ch \<pi> x\<rbrace>" by (simp add: Chan)
 
   from `(\<V>, \<C>) \<Turnstile>\<^sub>\<sigma> \<langle>LET x = CHAN \<lparr>\<rparr> in e; \<rho>; \<kappa>\<rangle>` 
-  have "(\<V>, \<C>) \<Turnstile>\<^sub>\<rho> \<rho>" by (simp add: accept_state.simps)+
+  have "(\<V>, \<C>) \<Turnstile>\<^sub>\<rho> \<rho>" by (simp add: static_eval_state.simps)+
   {
     fix x' \<omega>'
     assume "(\<rho>(x \<mapsto> \<lbrace>Ch \<pi> x\<rbrace>)) x' = Some \<omega>'" and "x \<noteq> x'"then
@@ -1266,23 +1266,23 @@ proof
 qed
 
 
-lemma accept_preserved_under_chan: "
+lemma static_eval_preserved_under_chan: "
   (\<V>, \<C>) \<Turnstile>\<^sub>\<E> \<E> \<Longrightarrow>
   \<E> \<pi> = Some (\<langle>LET x = CHAN \<lparr>\<rparr> in e; \<rho>; \<kappa>\<rangle>) \<Longrightarrow> 
   (\<V>, \<C>) \<Turnstile>\<^sub>\<E> \<E>(\<pi> ;; `x \<mapsto> \<langle>e; \<rho>(x \<mapsto> \<lbrace>Ch \<pi> x\<rbrace>); \<kappa>\<rangle>)
 "
 proof
   assume "(\<V>, \<C>) \<Turnstile>\<^sub>\<E> \<E>" and "\<E> \<pi> = Some (\<langle>LET x = CHAN \<lparr>\<rparr> in e; \<rho>; \<kappa>\<rangle>)" then
-  have "(\<V>, \<C>) \<Turnstile>\<^sub>e e" by (blast intro: accept_pool_to_exp_let)
+  have "(\<V>, \<C>) \<Turnstile>\<^sub>e e" by (blast intro: static_eval_pool_to_exp_let)
 
   from `(\<V>, \<C>) \<Turnstile>\<^sub>\<E> \<E>` and `\<E> \<pi> = Some (\<langle>LET x = CHAN \<lparr>\<rparr> in e; \<rho>; \<kappa>\<rangle>)`
-  have "(\<V>, \<C>) \<Turnstile>\<^sub>\<rho> \<rho>(x \<mapsto> \<lbrace>Ch \<pi> x\<rbrace>)" by (blast intro: accept_pool_to_env_let_chan )
+  have "(\<V>, \<C>) \<Turnstile>\<^sub>\<rho> \<rho>(x \<mapsto> \<lbrace>Ch \<pi> x\<rbrace>)" by (blast intro: static_eval_pool_to_env_let_chan )
 
   from `(\<V>, \<C>) \<Turnstile>\<^sub>\<E> \<E>` and `\<E> \<pi> = Some (\<langle>LET x = CHAN \<lparr>\<rparr> in e; \<rho>; \<kappa>\<rangle>)`
-  have "(\<V>, \<C>) \<Turnstile>\<^sub>\<kappa> \<V> (\<lfloor>e\<rfloor>) \<Rrightarrow> \<kappa>" by (blast intro: accept_pool_to_stack_let)
+  have "(\<V>, \<C>) \<Turnstile>\<^sub>\<kappa> \<V> (\<lfloor>e\<rfloor>) \<Rrightarrow> \<kappa>" by (blast intro: static_eval_pool_to_stack_let)
 
   from `(\<V>, \<C>) \<Turnstile>\<^sub>e e` and `(\<V>, \<C>) \<Turnstile>\<^sub>\<rho> \<rho>(x \<mapsto> \<lbrace>Ch \<pi> x\<rbrace>)` and `(\<V>, \<C>) \<Turnstile>\<^sub>\<kappa> \<V> (\<lfloor>e\<rfloor>) \<Rrightarrow> \<kappa>`
-  have "(\<V>, \<C>) \<Turnstile>\<^sub>\<sigma> \<langle>e;\<rho>(x \<mapsto> \<lbrace>Ch \<pi> x\<rbrace>);\<kappa>\<rangle>" by (blast intro: accept_state.intros)
+  have "(\<V>, \<C>) \<Turnstile>\<^sub>\<sigma> \<langle>e;\<rho>(x \<mapsto> \<lbrace>Ch \<pi> x\<rbrace>);\<kappa>\<rangle>" by (blast intro: static_eval_state.intros)
   {
     fix \<pi>' \<sigma>'
     assume "(\<E>(\<pi> ;; `x \<mapsto> \<langle>e;\<rho>(x \<mapsto> \<lbrace>Ch \<pi> x\<rbrace>);\<kappa>\<rangle>)) \<pi>' = Some \<sigma>'" 
@@ -1294,7 +1294,7 @@ proof
 qed
 
 
-lemma accept_pool_to_env_let_spawn: "
+lemma static_eval_pool_to_env_let_spawn: "
   (\<V>, \<C>) \<Turnstile>\<^sub>\<E> \<E> \<Longrightarrow>
   \<E> \<pi> = Some (\<langle>LET x = SPAWN e\<^sub>c in e; \<rho>; \<kappa>\<rangle>) \<Longrightarrow> 
   (\<V>, \<C>) \<Turnstile>\<^sub>\<rho> \<rho>(x \<mapsto> \<lbrace>\<rbrace>)"
@@ -1302,12 +1302,12 @@ proof
 
   assume "(\<V>, \<C>) \<Turnstile>\<^sub>\<E> \<E>" and "\<E> \<pi> = Some (\<langle>LET x = SPAWN e\<^sub>c in e; \<rho>; \<kappa>\<rangle>)" then
   have "(\<V>, \<C>) \<Turnstile>\<^sub>\<sigma> \<langle>LET x = SPAWN e\<^sub>c in e; \<rho>; \<kappa>\<rangle>" by (simp add: static_eval_pool.simps) then
-  have "(\<V>, \<C>) \<Turnstile>\<^sub>e LET x = SPAWN e\<^sub>c in e" by (blast intro: accept_state.cases) then
+  have "(\<V>, \<C>) \<Turnstile>\<^sub>e LET x = SPAWN e\<^sub>c in e" by (blast intro: static_eval_state.cases) then
   have "{^\<lparr>\<rparr>} \<subseteq> \<V> x"  by (blast intro: static_eval.cases) then
   have "(\<V>, \<C>) \<Turnstile>\<^sub>\<omega> \<lbrace>\<rbrace>" by (simp add: Unit)
 
   from `(\<V>, \<C>) \<Turnstile>\<^sub>\<sigma> \<langle>LET x = SPAWN e\<^sub>c in e; \<rho>; \<kappa>\<rangle>` 
-  have "(\<V>, \<C>) \<Turnstile>\<^sub>\<rho> \<rho>" by (simp add: accept_state.simps)
+  have "(\<V>, \<C>) \<Turnstile>\<^sub>\<rho> \<rho>" by (simp add: static_eval_state.simps)
 
   {
     fix x' \<omega>'
@@ -1318,7 +1318,7 @@ proof
   show "\<forall>x' \<omega>'. (\<rho>(x \<mapsto> \<lbrace>\<rbrace>)) x' = Some \<omega>' \<longrightarrow> {|\<omega>'|} \<subseteq> \<V> x' \<and> (\<V>, \<C>) \<Turnstile>\<^sub>\<omega> \<omega>'" by simp
 qed
 
-lemma accept_preserved_under_spawn: "
+lemma static_eval_preserved_under_spawn: "
   (\<V>, \<C>) \<Turnstile>\<^sub>\<E> \<E> \<Longrightarrow>
   \<E> \<pi> = Some (\<langle>LET x = SPAWN e\<^sub>c in e; \<rho>; \<kappa>\<rangle>) \<Longrightarrow> 
   (\<V>, \<C>) \<Turnstile>\<^sub>\<E> \<E>(\<pi> ;; `x \<mapsto> \<langle>e; \<rho>(x \<mapsto> \<lbrace>\<rbrace>); \<kappa>\<rangle>, \<pi>;;.x \<mapsto> \<langle>e\<^sub>c; \<rho>; []\<rangle>)
@@ -1328,27 +1328,27 @@ proof
   assume "(\<V>, \<C>) \<Turnstile>\<^sub>\<E> \<E>" and "\<E> \<pi> = Some (\<langle>LET x = SPAWN e\<^sub>c in e; \<rho>; \<kappa>\<rangle>)"
 
   from `(\<V>, \<C>) \<Turnstile>\<^sub>\<E> \<E>` and `\<E> \<pi> = Some (\<langle>LET x = SPAWN e\<^sub>c in e; \<rho>; \<kappa>\<rangle>)`
-  have "(\<V>, \<C>) \<Turnstile>\<^sub>e e" by (blast intro: accept_pool_to_exp_let)
+  have "(\<V>, \<C>) \<Turnstile>\<^sub>e e" by (blast intro: static_eval_pool_to_exp_let)
 
   from `(\<V>, \<C>) \<Turnstile>\<^sub>\<E> \<E>` and `\<E> \<pi> = Some (\<langle>LET x = SPAWN e\<^sub>c in e; \<rho>; \<kappa>\<rangle>)`
-  have "(\<V>, \<C>) \<Turnstile>\<^sub>\<rho> \<rho>(x \<mapsto> \<lbrace>\<rbrace>)" by (blast intro: accept_pool_to_env_let_spawn)
+  have "(\<V>, \<C>) \<Turnstile>\<^sub>\<rho> \<rho>(x \<mapsto> \<lbrace>\<rbrace>)" by (blast intro: static_eval_pool_to_env_let_spawn)
 
   from `(\<V>, \<C>) \<Turnstile>\<^sub>\<E> \<E>` and `\<E> \<pi> = Some (\<langle>LET x = SPAWN e\<^sub>c in e; \<rho>; \<kappa>\<rangle>)`
-  have "(\<V>, \<C>) \<Turnstile>\<^sub>\<kappa> \<V> (\<lfloor>e\<rfloor>) \<Rrightarrow> \<kappa>" by (blast intro: accept_pool_to_stack_let)
+  have "(\<V>, \<C>) \<Turnstile>\<^sub>\<kappa> \<V> (\<lfloor>e\<rfloor>) \<Rrightarrow> \<kappa>" by (blast intro: static_eval_pool_to_stack_let)
 
   from \<open>(\<V>, \<C>) \<Turnstile>\<^sub>\<kappa> \<V> (\<lfloor>e\<rfloor>) \<Rrightarrow> \<kappa>\<close> \<open>(\<V>, \<C>) \<Turnstile>\<^sub>\<rho> \<rho>(x \<mapsto> \<lbrace>\<rbrace>)\<close> \<open>(\<V>, \<C>) \<Turnstile>\<^sub>e e\<close>
-  have "(\<V>, \<C>) \<Turnstile>\<^sub>\<sigma> \<langle>e;\<rho>(x \<mapsto> \<lbrace>\<rbrace>);\<kappa>\<rangle>" by (simp add: accept_state.intros)
+  have "(\<V>, \<C>) \<Turnstile>\<^sub>\<sigma> \<langle>e;\<rho>(x \<mapsto> \<lbrace>\<rbrace>);\<kappa>\<rangle>" by (simp add: static_eval_state.intros)
 
   from `(\<V>, \<C>) \<Turnstile>\<^sub>\<E> \<E>` and `\<E> \<pi> = Some (\<langle>LET x = SPAWN e\<^sub>c in e; \<rho>; \<kappa>\<rangle>)`
   have "(\<V>, \<C>) \<Turnstile>\<^sub>\<sigma> \<langle>LET x = SPAWN e\<^sub>c in e; \<rho>; \<kappa>\<rangle>" by (simp add: static_eval_pool.simps) then
-  have "(\<V>, \<C>) \<Turnstile>\<^sub>e LET x = SPAWN e\<^sub>c in e" and "(\<V>, \<C>) \<Turnstile>\<^sub>\<rho> \<rho>" by (simp add: accept_state.simps)+
+  have "(\<V>, \<C>) \<Turnstile>\<^sub>e LET x = SPAWN e\<^sub>c in e" and "(\<V>, \<C>) \<Turnstile>\<^sub>\<rho> \<rho>" by (simp add: static_eval_state.simps)+
   
   from `(\<V>, \<C>) \<Turnstile>\<^sub>e LET x = SPAWN e\<^sub>c in e`
   have "(\<V>, \<C>) \<Turnstile>\<^sub>e e\<^sub>c" by (blast intro: static_eval.cases)
 
   have "(\<V>, \<C>) \<Turnstile>\<^sub>\<kappa> \<V> (\<lfloor>e\<^sub>c\<rfloor>) \<Rrightarrow> []" by (simp add: static_eval_stack.Empty)
   from \<open>(\<V>, \<C>) \<Turnstile>\<^sub>\<kappa> \<V> (\<lfloor>e\<^sub>c\<rfloor>) \<Rrightarrow> []\<close> \<open>(\<V>, \<C>) \<Turnstile>\<^sub>\<rho> \<rho>\<close> \<open>(\<V>, \<C>) \<Turnstile>\<^sub>e e\<^sub>c\<close> 
-  have "(\<V>, \<C>) \<Turnstile>\<^sub>\<sigma> \<langle>e\<^sub>c;\<rho>;[]\<rangle>" by (simp add: accept_state.intros)
+  have "(\<V>, \<C>) \<Turnstile>\<^sub>\<sigma> \<langle>e\<^sub>c;\<rho>;[]\<rangle>" by (simp add: static_eval_state.intros)
 
   {
     fix \<pi>' \<sigma>'
@@ -1361,7 +1361,7 @@ proof
 qed
 
 
-theorem accept_preserved_under_concur_step : "
+theorem static_eval_preserved_under_concur_step : "
   \<lbrakk>
     (\<V>, \<C>) \<Turnstile>\<^sub>\<E> \<E>; 
     \<E> \<rightarrow> \<E>'
@@ -1378,7 +1378,7 @@ proof -
     assume "leaf \<E> \<pi>" and "\<E> \<pi> = Some (\<langle>RESULT x;\<rho>;\<langle>x\<^sub>\<kappa>,e\<^sub>\<kappa>,\<rho>\<^sub>\<kappa>\<rangle> # \<kappa>\<rangle>)"
     and "\<langle>RESULT x;\<rho>;\<langle>x\<^sub>\<kappa>,e\<^sub>\<kappa>,\<rho>\<^sub>\<kappa>\<rangle> # \<kappa>\<rangle> \<hookrightarrow> \<sigma>'"
     with \<open>(\<V>, \<C>) \<Turnstile>\<^sub>\<E> \<E>\<close>
-    have "(\<V>, \<C>) \<Turnstile>\<^sub>\<E> \<E>(\<pi> ;; \<downharpoonleft>x\<^sub>\<kappa> \<mapsto> \<sigma>')" by (simp add:  accept_preserved_under_seq_step_down)
+    have "(\<V>, \<C>) \<Turnstile>\<^sub>\<E> \<E>(\<pi> ;; \<downharpoonleft>x\<^sub>\<kappa> \<mapsto> \<sigma>')" by (simp add:  static_eval_preserved_under_seq_step_down)
     with `\<E>' = \<E> ++ [\<pi> ;; \<downharpoonleft>x\<^sub>\<kappa> \<mapsto> \<sigma>']`
     show "(\<V>, \<C>) \<Turnstile>\<^sub>\<E> \<E>'" by simp
   next
@@ -1387,7 +1387,7 @@ proof -
     assume "leaf \<E> \<pi>" and "\<E> \<pi> = Some (\<langle>LET x = b in e;\<rho>;\<kappa>\<rangle>)"
     and "\<langle>LET x = b in e;\<rho>;\<kappa>\<rangle> \<hookrightarrow> \<langle>e';\<rho>';\<kappa>\<rangle>"
     with \<open>(\<V>, \<C>) \<Turnstile>\<^sub>\<E> \<E>\<close>
-    have "(\<V>, \<C>) \<Turnstile>\<^sub>\<E> \<E>(\<pi> ;; `x \<mapsto> \<langle>e';\<rho>';\<kappa>\<rangle>)" by (simp add: accept_preserved_under_seq_step)
+    have "(\<V>, \<C>) \<Turnstile>\<^sub>\<E> \<E>(\<pi> ;; `x \<mapsto> \<langle>e';\<rho>';\<kappa>\<rangle>)" by (simp add: static_eval_preserved_under_seq_step)
     with \<open>\<E>' = \<E> ++ [\<pi> ;; `x \<mapsto> \<langle>e';\<rho>';\<kappa>\<rangle>]\<close>
     show "(\<V>, \<C>) \<Turnstile>\<^sub>\<E> \<E>'" by simp
   next
@@ -1396,7 +1396,7 @@ proof -
     assume "leaf \<E> \<pi>" and "\<E> \<pi> = Some (\<langle>LET x = b in e;\<rho>;\<kappa>\<rangle>)"
     and "\<langle>LET x = b in e;\<rho>;\<kappa>\<rangle> \<hookrightarrow> \<langle>e';\<rho>';\<langle>x,e,\<rho>\<rangle> # \<kappa>\<rangle>"
     with \<open>(\<V>, \<C>) \<Turnstile>\<^sub>\<E> \<E>\<close>
-    have "(\<V>, \<C>) \<Turnstile>\<^sub>\<E> \<E>(\<pi> ;; \<upharpoonleft>x \<mapsto> \<langle>e';\<rho>';\<langle>x,e,\<rho>\<rangle> # \<kappa>\<rangle>)" by (simp add: accept_preserved_under_seq_step_up)
+    have "(\<V>, \<C>) \<Turnstile>\<^sub>\<E> \<E>(\<pi> ;; \<upharpoonleft>x \<mapsto> \<langle>e';\<rho>';\<langle>x,e,\<rho>\<rangle> # \<kappa>\<rangle>)" by (simp add: static_eval_preserved_under_seq_step_up)
     with \<open>\<E>' = \<E> ++ [\<pi> ;; \<upharpoonleft>x \<mapsto> \<langle>e';\<rho>';\<langle>x,e,\<rho>\<rangle> # \<kappa>\<rangle>]\<close>
     show "(\<V>, \<C>) \<Turnstile>\<^sub>\<E> \<E>'" by simp
   next
@@ -1404,7 +1404,7 @@ proof -
     assume "\<E>' = \<E> ++ [\<pi> ;; `x \<mapsto> \<langle>e;\<rho> ++ [x \<mapsto> \<lbrace>Ch \<pi> x\<rbrace>];\<kappa>\<rangle>]"
     assume "leaf \<E> \<pi>" and "\<E> \<pi> = Some (\<langle>LET x = CHAN \<lparr>\<rparr> in e;\<rho>;\<kappa>\<rangle>)"
     with \<open>(\<V>, \<C>) \<Turnstile>\<^sub>\<E> \<E>\<close>
-    have "(\<V>, \<C>) \<Turnstile>\<^sub>\<E> \<E>(\<pi> ;; `x \<mapsto> \<langle>e;\<rho> ++ [x \<mapsto> \<lbrace>Ch \<pi> x\<rbrace>];\<kappa>\<rangle>)" by (simp add: accept_preserved_under_chan)
+    have "(\<V>, \<C>) \<Turnstile>\<^sub>\<E> \<E>(\<pi> ;; `x \<mapsto> \<langle>e;\<rho> ++ [x \<mapsto> \<lbrace>Ch \<pi> x\<rbrace>];\<kappa>\<rangle>)" by (simp add: static_eval_preserved_under_chan)
     with \<open>\<E>' = \<E> ++ [\<pi> ;; `x \<mapsto> \<langle>e;\<rho> ++ [x \<mapsto> \<lbrace>Ch \<pi> x\<rbrace>];\<kappa>\<rangle>]\<close>
     show "(\<V>, \<C>) \<Turnstile>\<^sub>\<E> \<E>'" by simp
   next
@@ -1412,7 +1412,7 @@ proof -
     assume "\<E>' = \<E> ++ [\<pi> ;; `x \<mapsto> \<langle>e;\<rho> ++ [x \<mapsto> \<lbrace>\<rbrace>];\<kappa>\<rangle>, \<pi> ;; .x \<mapsto> \<langle>e\<^sub>c;\<rho>;[]\<rangle>]"
     assume "leaf \<E> \<pi>" and "\<E> \<pi> = Some (\<langle>LET x = SPAWN e\<^sub>c in e;\<rho>;\<kappa>\<rangle>)"
     with \<open>(\<V>, \<C>) \<Turnstile>\<^sub>\<E> \<E>\<close>
-    have "(\<V>, \<C>) \<Turnstile>\<^sub>\<E> \<E>(\<pi> ;; `x \<mapsto> \<langle>e;\<rho> ++ [x \<mapsto> \<lbrace>\<rbrace>];\<kappa>\<rangle>, \<pi> ;; .x \<mapsto> \<langle>e\<^sub>c;\<rho>;[]\<rangle>)" by (simp add: accept_preserved_under_spawn)
+    have "(\<V>, \<C>) \<Turnstile>\<^sub>\<E> \<E>(\<pi> ;; `x \<mapsto> \<langle>e;\<rho> ++ [x \<mapsto> \<lbrace>\<rbrace>];\<kappa>\<rangle>, \<pi> ;; .x \<mapsto> \<langle>e\<^sub>c;\<rho>;[]\<rangle>)" by (simp add: static_eval_preserved_under_spawn)
     with \<open>\<E>' = \<E> ++ [\<pi> ;; `x \<mapsto> \<langle>e;\<rho> ++ [x \<mapsto> \<lbrace>\<rbrace>];\<kappa>\<rangle>, \<pi> ;; .x \<mapsto> \<langle>e\<^sub>c;\<rho>;[]\<rangle>]\<close>
     show "(\<V>, \<C>) \<Turnstile>\<^sub>\<E> \<E>'" by simp
   next
@@ -1429,14 +1429,14 @@ proof -
     and "\<rho>\<^sub>r\<^sub>e x\<^sub>r\<^sub>c = Some \<lbrace>c\<rbrace>"
     and "\<rho>\<^sub>s\<^sub>e x\<^sub>m = Some \<omega>\<^sub>m"
     with \<open>(\<V>, \<C>) \<Turnstile>\<^sub>\<E> \<E>\<close>
-    have "(\<V>, \<C>) \<Turnstile>\<^sub>\<E> \<E>(\<pi>\<^sub>s ;; `x\<^sub>s \<mapsto> \<langle>e\<^sub>s;\<rho>\<^sub>s ++ [x\<^sub>s \<mapsto> \<lbrace>\<rbrace>];\<kappa>\<^sub>s\<rangle>, \<pi>\<^sub>r ;; `x\<^sub>r \<mapsto> \<langle>e\<^sub>r;\<rho>\<^sub>r ++ [x\<^sub>r \<mapsto> \<omega>\<^sub>m];\<kappa>\<^sub>r\<rangle>)" by (simp add: accept_preserved_under_sync)
+    have "(\<V>, \<C>) \<Turnstile>\<^sub>\<E> \<E>(\<pi>\<^sub>s ;; `x\<^sub>s \<mapsto> \<langle>e\<^sub>s;\<rho>\<^sub>s ++ [x\<^sub>s \<mapsto> \<lbrace>\<rbrace>];\<kappa>\<^sub>s\<rangle>, \<pi>\<^sub>r ;; `x\<^sub>r \<mapsto> \<langle>e\<^sub>r;\<rho>\<^sub>r ++ [x\<^sub>r \<mapsto> \<omega>\<^sub>m];\<kappa>\<^sub>r\<rangle>)" by (simp add: static_eval_preserved_under_sync)
     with \<open>\<E>' = \<E> ++ [\<pi>\<^sub>s ;; `x\<^sub>s \<mapsto> \<langle>e\<^sub>s;\<rho>\<^sub>s ++ [x\<^sub>s \<mapsto> \<lbrace>\<rbrace>];\<kappa>\<^sub>s\<rangle>, \<pi>\<^sub>r ;; `x\<^sub>r \<mapsto> \<langle>e\<^sub>r;\<rho>\<^sub>r ++ [x\<^sub>r \<mapsto> \<omega>\<^sub>m];\<kappa>\<^sub>r\<rangle>]\<close>
     show "(\<V>, \<C>) \<Turnstile>\<^sub>\<E> \<E>'" by simp
   qed
 qed
 
 
-theorem accept_preserved_under_concur_step_star : "
+theorem static_eval_preserved_under_concur_step_star : "
   \<lbrakk>
     (\<V>, \<C>) \<Turnstile>\<^sub>\<E> \<E>;  
     \<E> \<rightarrow>* \<E>'
@@ -1454,12 +1454,12 @@ proof -
     case (step \<E> \<E>\<^sub>m \<E>')
     assume " \<E> \<rightarrow> \<E>\<^sub>m"
     and "(\<V>, \<C>) \<Turnstile>\<^sub>\<E> \<E>\<^sub>m \<longrightarrow> (\<V>, \<C>) \<Turnstile>\<^sub>\<E> \<E>'" then
-    show "(\<V>, \<C>) \<Turnstile>\<^sub>\<E> \<E> \<longrightarrow> (\<V>, \<C>) \<Turnstile>\<^sub>\<E> \<E>'" by (blast intro: accept_preserved_under_concur_step)
+    show "(\<V>, \<C>) \<Turnstile>\<^sub>\<E> \<E> \<longrightarrow> (\<V>, \<C>) \<Turnstile>\<^sub>\<E> \<E>'" by (blast intro: static_eval_preserved_under_concur_step)
   qed with `(\<V>, \<C>) \<Turnstile>\<^sub>\<E> \<E>`
   show "(\<V>, \<C>) \<Turnstile>\<^sub>\<E> \<E>'" by blast
 qed
 
-theorem accept_env_to_precise : "
+theorem static_eval_env_to_precise : "
   (\<V>, \<C>) \<Turnstile>\<^sub>\<rho> \<rho>
   \<Longrightarrow>
   \<parallel>\<rho>\<parallel> \<sqsubseteq> \<V>
@@ -1476,7 +1476,7 @@ proof -
   show "\<parallel>\<rho>\<parallel> \<sqsubseteq> \<V>" by (simp add: abstract_value_env_precision_def)
 qed
 
-theorem accept_pool_to_precise : "
+theorem static_eval_pool_to_precise : "
   \<lbrakk>
     (\<V>, \<C>) \<Turnstile>\<^sub>\<E> \<E>;
     \<E> \<pi> = Some (\<langle>e; \<rho>; \<kappa>\<rangle>)
@@ -1487,11 +1487,11 @@ theorem accept_pool_to_precise : "
 proof -
   assume "(\<V>, \<C>) \<Turnstile>\<^sub>\<E> \<E>" and "\<E> \<pi> = Some (\<langle>e; \<rho>; \<kappa>\<rangle>)" then
   have "(\<V>, \<C>) \<Turnstile>\<^sub>\<sigma> \<langle>e; \<rho>; \<kappa>\<rangle>" by (simp add: static_eval_pool.simps) then
-  have "(\<V>, \<C>) \<Turnstile>\<^sub>\<rho> \<rho>" by (simp add: accept_state.simps) then
-  show "\<parallel>\<rho>\<parallel> \<sqsubseteq> \<V>"  by (simp add: accept_env_to_precise)
+  have "(\<V>, \<C>) \<Turnstile>\<^sub>\<rho> \<rho>" by (simp add: static_eval_state.simps) then
+  show "\<parallel>\<rho>\<parallel> \<sqsubseteq> \<V>"  by (simp add: static_eval_env_to_precise)
 qed
 
-theorem accept_pool_sound : "
+theorem isnt_static_eval_pool_sound : "
   \<lbrakk>
     (\<V>, \<C>) \<Turnstile>\<^sub>\<E> \<E>; 
     \<E> \<rightarrow>* \<E>';
@@ -1501,9 +1501,9 @@ theorem accept_pool_sound : "
 "
 proof -
   assume "(\<V>, \<C>) \<Turnstile>\<^sub>\<E> \<E>" and "\<E> \<rightarrow>* \<E>'" and "\<E>' \<pi> = Some (\<langle>e'; \<rho>'; \<kappa>'\<rangle>)" then
-  have "(\<V>, \<C>) \<Turnstile>\<^sub>\<E> \<E>'" by (blast intro: accept_preserved_under_concur_step_star)
+  have "(\<V>, \<C>) \<Turnstile>\<^sub>\<E> \<E>'" by (blast intro: static_eval_preserved_under_concur_step_star)
   with \<open>\<E>' \<pi> = Some (\<langle>e';\<rho>';\<kappa>'\<rangle>)\<close>
-  show "\<parallel>\<rho>'\<parallel> \<sqsubseteq> \<V>" by (blast intro: accept_pool_to_precise)
+  show "\<parallel>\<rho>'\<parallel> \<sqsubseteq> \<V>" by (blast intro: static_eval_pool_to_precise)
 qed
 
 
@@ -1520,7 +1520,7 @@ proof -
   have "(\<V>, \<C>) \<Turnstile>\<^sub>\<kappa> \<V> (\<lfloor>e\<rfloor>) \<Rrightarrow> []" by (simp add: static_eval_stack.Empty)
 
   from `(\<V>, \<C>) \<Turnstile>\<^sub>e e` and `(\<V>, \<C>) \<Turnstile>\<^sub>\<rho> empty` and `(\<V>, \<C>) \<Turnstile>\<^sub>\<kappa> \<V> (\<lfloor>e\<rfloor>) \<Rrightarrow> []`
-  have "(\<V>, \<C>) \<Turnstile>\<^sub>\<sigma> \<langle>e; empty; []\<rangle>" by (simp add: accept_state.intros)
+  have "(\<V>, \<C>) \<Turnstile>\<^sub>\<sigma> \<langle>e; empty; []\<rangle>" by (simp add: static_eval_state.intros)
 
   have "[[] \<mapsto> \<langle>e; empty; []\<rangle>] [] = Some (\<langle>e; empty; []\<rangle>)" by simp
   with `(\<V>, \<C>) \<Turnstile>\<^sub>\<sigma> \<langle>e; empty; []\<rangle>`
@@ -1528,7 +1528,7 @@ proof -
 qed
 
 
-theorem isnt_abstract_value_sound : "
+theorem isnt_static_eval_sound : "
   \<lbrakk>
     (\<V>, \<C>) \<Turnstile>\<^sub>e e; 
     [[] \<mapsto> \<langle>e; empty; []\<rangle>] \<rightarrow>* \<E>';
@@ -1544,7 +1544,7 @@ proof -
   have "(\<V>, \<C>) \<Turnstile>\<^sub>\<E> [[] \<mapsto> \<langle>e; empty; []\<rangle>]" by (simp add: static_eval_to_pool)
 
   from \<open>(\<V>, \<C>) \<Turnstile>\<^sub>\<E> [[] \<mapsto> \<langle>e;Map.empty;[]\<rangle>]\<close> \<open>[[] \<mapsto> \<langle>e;Map.empty;[]\<rangle>] \<rightarrow>* \<E>'\<close> \<open>\<E>' \<pi> = Some (\<langle>e';\<rho>';\<kappa>'\<rangle>)\<close>
-  show "\<parallel>\<rho>'\<parallel> \<sqsubseteq> \<V>" by (simp add: accept_pool_sound)
+  show "\<parallel>\<rho>'\<parallel> \<sqsubseteq> \<V>" by (simp add: isnt_static_eval_pool_sound)
 qed
 
 
@@ -1564,7 +1564,7 @@ proof -
   show "{|\<omega>|} \<subseteq> \<V> x" by (simp add: env_to_abstract_value_env_def)
 qed
 
-corollary isnt_abstract_value_sound_coro: "
+corollary isnt_static_eval_sound_coro: "
   \<lbrakk>
     (\<V>, \<C>) \<Turnstile>\<^sub>e e ;
     [[] \<mapsto> \<langle>e;Map.empty;[]\<rangle>] \<rightarrow>* \<E>';
@@ -1578,7 +1578,7 @@ proof -
   assume "(\<V>, \<C>) \<Turnstile>\<^sub>e e"
   and "[[] \<mapsto> \<langle>e;Map.empty;[]\<rangle>] \<rightarrow>* \<E>'"
   and "\<E>' \<pi> = Some (\<langle>e';\<rho>';\<kappa>'\<rangle>)" then
-  have "\<parallel>\<rho>'\<parallel> \<sqsubseteq> \<V>" by (simp add: isnt_abstract_value_sound)
+  have "\<parallel>\<rho>'\<parallel> \<sqsubseteq> \<V>" by (simp add: isnt_static_eval_sound)
   with `\<rho>' x = Some \<omega>`
   show "{|\<omega>|} \<subseteq> \<V> x" using abstracted_value_exists by blast
 qed
