theory/Sound_Traceability.thy
@@ -6,7 +6,7 @@ theory Sound_Traceability
 begin
 
 
-inductive stack_traceable :: "abstract_value_env \<Rightarrow> exp \<Rightarrow> control_path \<Rightarrow> cont list \<Rightarrow> bool" ("_ \<tturnstile> _ \<down> _ \<mapsto> _" [56,0,0,56]55)  where
+inductive stack_static_traceable :: "abstract_value_env \<Rightarrow> exp \<Rightarrow> control_path \<Rightarrow> cont list \<Rightarrow> bool" ("_ \<tturnstile> _ \<down> _ \<mapsto> _" [56,0,0,56]55)  where
   Empty: "
     \<lbrakk> 
       \<downharpoonright>\<pi>\<upharpoonleft>
@@ -33,24 +33,24 @@ lemma singleton_eq_empty_surround: "
 "
 by simp
 
-lemma stack_traceable_preserved_over_balanced_extension:
+lemma stack_static_traceable_preserved_over_balanced_extension:
   "\<V> \<tturnstile> e\<^sub>0 \<down> \<pi> \<mapsto> \<kappa> \<Longrightarrow> \<downharpoonright>\<pi>'\<upharpoonleft> \<Longrightarrow> \<V> \<tturnstile> e\<^sub>0 \<down> \<pi> @ \<pi>' \<mapsto> \<kappa>" 
 proof -
   assume "\<V> \<tturnstile> e\<^sub>0 \<down> \<pi> \<mapsto> \<kappa>" "\<downharpoonright>\<pi>'\<upharpoonleft>" then 
   show "\<V> \<tturnstile> e\<^sub>0 \<down> \<pi> @ \<pi>' \<mapsto> \<kappa>"
-  proof (cases rule: stack_traceable.cases)
+  proof (cases rule: stack_static_traceable.cases)
     case Empty assume "\<kappa> = []" "\<downharpoonright>\<pi>\<upharpoonleft>"
     
     from `\<downharpoonright>\<pi>\<upharpoonleft>` `\<downharpoonright>\<pi>'\<upharpoonleft>`
     have "\<downharpoonright>(\<pi> @ \<pi>')\<upharpoonleft>" by (simp add: Append) then
-    have "\<V> \<tturnstile> e\<^sub>0 \<down> \<pi> @ \<pi>' \<mapsto> []" by (simp add: stack_traceable.Empty)
+    have "\<V> \<tturnstile> e\<^sub>0 \<down> \<pi> @ \<pi>' \<mapsto> []" by (simp add: stack_static_traceable.Empty)
     with `\<kappa> = []`
     show "\<V> \<tturnstile> e\<^sub>0 \<down> \<pi> @ \<pi>' \<mapsto> \<kappa>" by blast
   next
     case (Empty_Local \<pi>\<^sub>2 \<pi>\<^sub>1 x) assume "\<pi> = \<pi>\<^sub>1 @ .x # \<pi>\<^sub>2" "\<kappa> = []" "\<downharpoonright>\<pi>\<^sub>2\<upharpoonleft>"
     from `\<downharpoonright>\<pi>\<^sub>2\<upharpoonleft>` `\<downharpoonright>\<pi>'\<upharpoonleft>` 
     have "\<downharpoonright>(\<pi>\<^sub>2 @ \<pi>')\<upharpoonleft>" by (simp add: Append) then
-    have "\<V> \<tturnstile> e\<^sub>0 \<down> \<pi>\<^sub>1 @ .x # \<pi>\<^sub>2 @ \<pi>' \<mapsto> []" by (simp add: stack_traceable.Empty_Local)
+    have "\<V> \<tturnstile> e\<^sub>0 \<down> \<pi>\<^sub>1 @ .x # \<pi>\<^sub>2 @ \<pi>' \<mapsto> []" by (simp add: stack_static_traceable.Empty_Local)
     with `\<pi> = \<pi>\<^sub>1 @ .x # \<pi>\<^sub>2` `\<kappa> = []` 
     show "\<V> \<tturnstile> e\<^sub>0 \<down> \<pi> @ \<pi>' \<mapsto> \<kappa>" by simp
   next
@@ -62,23 +62,23 @@ proof -
     from `\<downharpoonright>\<pi>\<^sub>2\<upharpoonleft>` `\<downharpoonright>\<pi>'\<upharpoonleft>`
     have "\<downharpoonright>(\<pi>\<^sub>2 @ \<pi>')\<upharpoonleft>" by (simp add: Append)
     with `\<V> \<turnstile> e\<^sub>0 \<down> \<pi>\<^sub>1 \<mapsto> LET x\<^sub>\<kappa> = b in e\<^sub>\<kappa>` `\<V> \<tturnstile> e\<^sub>0 \<down> \<pi>\<^sub>1 \<mapsto> \<kappa>'`
-    have "\<V> \<tturnstile> e\<^sub>0 \<down> \<pi>\<^sub>1 @ \<upharpoonleft>x\<^sub>\<kappa> # \<pi>\<^sub>2 @ \<pi>' \<mapsto> \<langle>x\<^sub>\<kappa>,e\<^sub>\<kappa>,\<rho>\<^sub>\<kappa>\<rangle> # \<kappa>'" by (auto simp: stack_traceable.Nonempty)
+    have "\<V> \<tturnstile> e\<^sub>0 \<down> \<pi>\<^sub>1 @ \<upharpoonleft>x\<^sub>\<kappa> # \<pi>\<^sub>2 @ \<pi>' \<mapsto> \<langle>x\<^sub>\<kappa>,e\<^sub>\<kappa>,\<rho>\<^sub>\<kappa>\<rangle> # \<kappa>'" by (auto simp: stack_static_traceable.Nonempty)
     with `\<pi> = \<pi>\<^sub>1 @ \<upharpoonleft>x\<^sub>\<kappa> # \<pi>\<^sub>2` `\<kappa> = \<langle>x\<^sub>\<kappa>,e\<^sub>\<kappa>,\<rho>\<^sub>\<kappa>\<rangle> # \<kappa>'`
     show "\<V> \<tturnstile> e\<^sub>0 \<down> \<pi> @ \<pi>' \<mapsto> \<kappa>" by simp
   qed
 qed
 (*
-apply (erule stack_traceable.cases; auto)
-   apply (simp add: stack_traceable.Empty)
+apply (erule stack_static_traceable.cases; auto)
+   apply (simp add: stack_static_traceable.Empty)
   apply (simp add: Empty_Local)
- apply (simp add: stack_traceable.Nonempty)
+ apply (simp add: stack_static_traceable.Nonempty)
 done
 *)
 
-lemma stack_traceable_preserved_over_seq_extension:"
+lemma stack_static_traceable_preserved_over_seq_extension:"
   \<V> \<tturnstile> e\<^sub>0 \<down> \<pi> \<mapsto> \<kappa> \<Longrightarrow> \<V> \<tturnstile> e\<^sub>0 \<down> \<pi> ;; `x \<mapsto> \<kappa>
 "
-by (simp add: Linear stack_traceable_preserved_over_balanced_extension)
+by (simp add: Linear stack_static_traceable_preserved_over_balanced_extension)
 
 inductive subexp :: "exp \<Rightarrow> exp \<Rightarrow> bool" ("_ \<preceq>\<^sub>e _" [56,56]55) where
   Refl : "
@@ -171,7 +171,7 @@ lemma subexp1: "
 by (simp add: Let Refl)
 
 
-theorem traceable_implies_subexp: "
+theorem static_traceable_implies_subexp: "
   \<lbrakk>
     \<V> \<turnstile> e\<^sub>0 \<down> \<pi> \<mapsto> e;
     (\<forall> x \<omega> . |\<omega>| \<in> \<V> x \<longrightarrow> (\<exists> x e\<^sub>n . LET x = val_to_bind \<omega> in e\<^sub>n \<preceq>\<^sub>e e\<^sub>0))
@@ -182,7 +182,7 @@ proof -
   assume "\<forall>x \<omega>. |\<omega>| \<in> \<V> x \<longrightarrow> (\<exists>x e\<^sub>n. LET x = val_to_bind \<omega> in e\<^sub>n \<preceq>\<^sub>e e\<^sub>0)"
   assume "\<V> \<turnstile> e\<^sub>0 \<down> \<pi> \<mapsto> e" then
   have "(\<forall> x \<omega> . |\<omega>| \<in> \<V> x \<longrightarrow> (\<exists> x e\<^sub>n . LET x = val_to_bind \<omega> in e\<^sub>n \<preceq>\<^sub>e e\<^sub>0)) \<longrightarrow> e \<preceq>\<^sub>e e\<^sub>0"
-  proof (induction rule: traceable.induct)
+  proof (induction rule: static_traceable.induct)
     case (Start \<V> e\<^sub>0)
     then show ?case
     by (simp add: Refl)
@@ -364,7 +364,7 @@ inductive flow :: "(abstract_value_env \<times> flow_set) \<Rightarrow> exp \<Ri
   "
 
 
-lemma traceable_exp_preserved_sync_recv_evt: "
+lemma static_traceable_exp_preserved_sync_recv_evt: "
 \<lbrakk>
   \<forall>\<pi> e \<rho> \<kappa>. \<E> \<pi> = Some (\<langle>e;\<rho>;\<kappa>\<rangle>) \<longrightarrow> \<V> \<turnstile> e\<^sub>0 \<down> \<pi> \<mapsto> e;
   (\<V>, \<C>) \<Turnstile>\<^sub>\<E> \<E>(\<pi>\<^sub>s ;; `x\<^sub>s \<mapsto> \<langle>e\<^sub>s;\<rho>\<^sub>s(x\<^sub>s \<mapsto> \<lbrace>\<rbrace>);\<kappa>\<^sub>s\<rangle>, \<pi>\<^sub>r ;; `x\<^sub>r \<mapsto> \<langle>e';\<rho>\<^sub>r(x\<^sub>r \<mapsto> \<omega>\<^sub>m);\<kappa>'\<rangle>);
@@ -380,17 +380,17 @@ proof -
   have "(\<E>(\<pi>\<^sub>s ;; `x\<^sub>s \<mapsto> \<langle>e\<^sub>s;\<rho>\<^sub>s(x\<^sub>s \<mapsto> \<lbrace>\<rbrace>);\<kappa>\<^sub>s\<rangle>, \<pi>\<^sub>r ;; `x\<^sub>r \<mapsto> \<langle>e';\<rho>\<^sub>r(x\<^sub>r \<mapsto> \<omega>\<^sub>m);\<kappa>'\<rangle>)) (\<pi>\<^sub>r ;; `x\<^sub>r) 
       = Some (\<langle>e';\<rho>\<^sub>r(x\<^sub>r \<mapsto> \<omega>\<^sub>m);\<kappa>'\<rangle>)" by simp
   with \<open>(\<V>, \<C>) \<Turnstile>\<^sub>\<E> \<E>(\<pi>\<^sub>s ;; `x\<^sub>s \<mapsto> \<langle>e\<^sub>s;\<rho>\<^sub>s(x\<^sub>s \<mapsto> \<lbrace>\<rbrace>);\<kappa>\<^sub>s\<rangle>, \<pi>\<^sub>r ;; `x\<^sub>r \<mapsto> \<langle>e';\<rho>\<^sub>r(x\<^sub>r \<mapsto> \<omega>\<^sub>m);\<kappa>'\<rangle>)\<close>
-  have "\<parallel>\<rho>\<^sub>r(x\<^sub>r \<mapsto> \<omega>\<^sub>m)\<parallel> \<sqsubseteq> \<V>" by (blast intro: accept_pool_to_precise)
+  have "\<parallel>\<rho>\<^sub>r(x\<^sub>r \<mapsto> \<omega>\<^sub>m)\<parallel> \<sqsubseteq> \<V>" by (blast intro: static_eval_pool_to_precise)
 
   have "(\<rho>\<^sub>r(x\<^sub>r \<mapsto> \<omega>\<^sub>m)) x\<^sub>r = Some \<omega>\<^sub>m" by simp
   with `\<parallel>\<rho>\<^sub>r(x\<^sub>r \<mapsto> \<omega>\<^sub>m)\<parallel> \<sqsubseteq> \<V>`
   have "|\<omega>\<^sub>m| \<in> \<V> x\<^sub>r" using abstracted_value_exists by blast
   with \<open>\<V> \<turnstile> e\<^sub>0 \<down> \<pi>\<^sub>r \<mapsto> LET x\<^sub>r = SYNC x\<^sub>r\<^sub>e in e\<^sub>n\<close> 
-  show "\<V> \<turnstile> e\<^sub>0 \<down> \<pi>\<^sub>r ;; `x\<^sub>r \<mapsto> e\<^sub>n" by (blast intro: traceable.Let_Sync)
+  show "\<V> \<turnstile> e\<^sub>0 \<down> \<pi>\<^sub>r ;; `x\<^sub>r \<mapsto> e\<^sub>n" by (blast intro: static_traceable.Let_Sync)
 qed
 
 
-lemma traceable_exp_preserved_sync_send_evt: "
+lemma static_traceable_exp_preserved_sync_send_evt: "
 \<lbrakk>
   \<forall>\<pi> e \<rho> \<kappa>. \<E> \<pi> = Some (\<langle>e;\<rho>;\<kappa>\<rangle>) \<longrightarrow> \<V> \<turnstile> e\<^sub>0 \<down> \<pi> \<mapsto> e;
   \<E> \<pi>\<^sub>s = Some (\<langle>LET x\<^sub>s = SYNC x\<^sub>s\<^sub>e in e';\<rho>\<^sub>s;\<kappa>'\<rangle>);
@@ -410,18 +410,18 @@ proof -
   have "(\<E>(\<pi>\<^sub>s ;; `x\<^sub>s \<mapsto> \<langle>e';\<rho>\<^sub>s(x\<^sub>s \<mapsto> \<lbrace>\<rbrace>);\<kappa>'\<rangle>, \<pi>\<^sub>r ;; `x\<^sub>r \<mapsto> \<langle>e\<^sub>r;\<rho>\<^sub>r(x\<^sub>r \<mapsto> \<omega>\<^sub>m);\<kappa>\<^sub>r\<rangle>)) (\<pi>\<^sub>s ;; `x\<^sub>s) 
       = Some (\<langle>e';\<rho>\<^sub>s(x\<^sub>s \<mapsto> \<lbrace>\<rbrace>);\<kappa>'\<rangle>)" by simp
   with `\<pi>\<^sub>s \<noteq> \<pi>\<^sub>r` \<open>(\<V>, \<C>) \<Turnstile>\<^sub>\<E> \<E>(\<pi>\<^sub>s ;; `x\<^sub>s \<mapsto> \<langle>e';\<rho>\<^sub>s(x\<^sub>s \<mapsto> \<lbrace>\<rbrace>);\<kappa>'\<rangle>, \<pi>\<^sub>r ;; `x\<^sub>r \<mapsto> \<langle>e\<^sub>r;\<rho>\<^sub>r(x\<^sub>r \<mapsto> \<omega>\<^sub>m);\<kappa>\<^sub>r\<rangle>)\<close>
-  have "\<parallel>\<rho>\<^sub>s(x\<^sub>s \<mapsto> \<lbrace>\<rbrace>)\<parallel> \<sqsubseteq> \<V>" using accept_pool_to_precise by blast
+  have "\<parallel>\<rho>\<^sub>s(x\<^sub>s \<mapsto> \<lbrace>\<rbrace>)\<parallel> \<sqsubseteq> \<V>" using static_eval_pool_to_precise by blast
 
   have "(\<rho>\<^sub>s(x\<^sub>s \<mapsto> \<lbrace>\<rbrace>)) x\<^sub>s = Some \<lbrace>\<rbrace>" by simp
   with `\<parallel>\<rho>\<^sub>s(x\<^sub>s \<mapsto> \<lbrace>\<rbrace>)\<parallel> \<sqsubseteq> \<V>`
   have " |\<lbrace>\<rbrace>| \<in> \<V> x\<^sub>s" using abstracted_value_exists by fastforce
 
   from \<open>\<V> \<turnstile> e\<^sub>0 \<down> \<pi>\<^sub>s \<mapsto> LET x\<^sub>s = SYNC x\<^sub>s\<^sub>e in e'\<close> \<open>|\<lbrace>\<rbrace>| \<in> \<V> x\<^sub>s\<close>
-  show "\<V> \<turnstile> e\<^sub>0 \<down> \<pi>\<^sub>s ;; `x\<^sub>s \<mapsto> e'" using traceable.Let_Sync by blast
+  show "\<V> \<turnstile> e\<^sub>0 \<down> \<pi>\<^sub>s ;; `x\<^sub>s \<mapsto> e'" using static_traceable.Let_Sync by blast
 
 qed
 
-lemma traceable_exp_preserved_under_seq_step_down: "
+lemma static_traceable_exp_preserved_under_seq_step_down: "
   (\<E>(\<pi> ;; \<downharpoonleft>x\<^sub>\<kappa> \<mapsto> \<sigma>')) \<pi>' = Some (\<langle>e';\<rho>';\<kappa>'\<rangle>) \<Longrightarrow>
   (\<forall>\<pi> e \<rho> \<kappa>. \<E> \<pi> = Some (\<langle>e;\<rho>;\<kappa>\<rangle>) \<longrightarrow>
     \<V> \<turnstile> e\<^sub>0 \<down> \<pi> \<mapsto> e \<and> \<V> \<tturnstile> e\<^sub>0 \<down> \<pi> \<mapsto> \<kappa>
@@ -447,7 +447,7 @@ proof -
   where "\<pi> = \<pi>\<^sub>1 @ \<upharpoonleft>x\<^sub>\<kappa> # \<pi>\<^sub>2" 
   and "\<V> \<turnstile> e\<^sub>0 \<down> \<pi>\<^sub>1 \<mapsto> LET x\<^sub>\<kappa> = b in e\<^sub>\<kappa>"
   and "\<V> \<tturnstile> e\<^sub>0 \<down> \<pi>\<^sub>1 \<mapsto> \<kappa>" and "\<downharpoonright>\<pi>\<^sub>2\<upharpoonleft>"
-  by (blast intro: stack_traceable.cases)
+  by (blast intro: stack_static_traceable.cases)
 
   from `\<pi> = \<pi>\<^sub>1 @ \<upharpoonleft>x\<^sub>\<kappa> # \<pi>\<^sub>2` and `\<V> \<turnstile> e\<^sub>0 \<down> \<pi> \<mapsto> RESULT x`
   have "\<V> \<turnstile> e\<^sub>0 \<down> \<pi>\<^sub>1 @ \<upharpoonleft>x\<^sub>\<kappa> # \<pi>\<^sub>2 \<mapsto> RESULT x" by simp
@@ -459,7 +459,7 @@ proof -
   from `\<V> \<turnstile> e\<^sub>0 \<down> \<pi>\<^sub>1 @ \<upharpoonleft>x\<^sub>\<kappa> # \<pi>\<^sub>2 \<mapsto> RESULT x` 
   and `\<V> \<turnstile> e\<^sub>0 \<down> \<pi>\<^sub>1 \<mapsto> LET x\<^sub>\<kappa> = b in e\<^sub>\<kappa>`
   and `\<downharpoonright>\<pi>\<^sub>2\<upharpoonleft>`
-  have "\<V> \<turnstile> e\<^sub>0 \<down> \<pi>\<^sub>1 @ \<upharpoonleft>x\<^sub>\<kappa> # (\<pi>\<^sub>2 ;; \<downharpoonleft>x\<^sub>\<kappa>) \<mapsto> e\<^sub>\<kappa>" by (blast intro: traceable.Result)
+  have "\<V> \<turnstile> e\<^sub>0 \<down> \<pi>\<^sub>1 @ \<upharpoonleft>x\<^sub>\<kappa> # (\<pi>\<^sub>2 ;; \<downharpoonleft>x\<^sub>\<kappa>) \<mapsto> e\<^sub>\<kappa>" by (blast intro: static_traceable.Result)
 
   show "\<V> \<turnstile> e\<^sub>0 \<down> \<pi>' \<mapsto> e'"
   proof cases
@@ -483,7 +483,7 @@ proof -
   qed
 qed
 
-lemma traceable_exp_preserved_under_seq_step: "
+lemma static_traceable_exp_preserved_under_seq_step: "
   \<E> \<rightarrow> \<E>(\<pi> ;; `x \<mapsto> \<langle>e'';\<rho>'';\<kappa>\<rangle>) \<Longrightarrow>
   (\<E>(\<pi> ;; `x \<mapsto> \<langle>e'';\<rho>'';\<kappa>\<rangle>)) \<pi>' = Some (\<langle>e';\<rho>';\<kappa>'\<rangle>) \<Longrightarrow>
   \<forall>\<pi> e \<rho> \<kappa>. \<E> \<pi> = Some (\<langle>e;\<rho>;\<kappa>\<rangle>) \<longrightarrow> \<V> \<turnstile> e\<^sub>0 \<down> \<pi> \<mapsto> e \<and> \<V> \<tturnstile> e\<^sub>0 \<down> \<pi> \<mapsto> \<kappa> \<Longrightarrow>
@@ -497,10 +497,10 @@ proof -
   assume "\<forall>\<pi> e \<rho> \<kappa>. \<E> \<pi> = Some (\<langle>e;\<rho>;\<kappa>\<rangle>) \<longrightarrow> \<V> \<turnstile> e\<^sub>0 \<down> \<pi> \<mapsto> e \<and> \<V> \<tturnstile> e\<^sub>0 \<down> \<pi> \<mapsto> \<kappa>"
   and "\<langle>LET x = b in e;\<rho>;\<kappa>\<rangle> \<hookrightarrow> \<langle>e'';\<rho>'';\<kappa>\<rangle>"
   assume "\<E> \<rightarrow> \<E>(\<pi> ;; `x \<mapsto> \<langle>e'';\<rho>'';\<kappa>\<rangle>)" and "(\<V>, \<C>) \<Turnstile>\<^sub>\<E> \<E>" then
-  have "(\<V>, \<C>) \<Turnstile>\<^sub>\<E> \<E>(\<pi> ;; `x \<mapsto> \<langle>e'';\<rho>'';\<kappa>\<rangle>)" by (blast intro: accept_preserved_under_concur_step)
+  have "(\<V>, \<C>) \<Turnstile>\<^sub>\<E> \<E>(\<pi> ;; `x \<mapsto> \<langle>e'';\<rho>'';\<kappa>\<rangle>)" by (blast intro: static_eval_preserved_under_concur_step)
 
   from \<open>(\<V>, \<C>) \<Turnstile>\<^sub>\<E> \<E>(\<pi> ;; `x \<mapsto> \<langle>e'';\<rho>'';\<kappa>\<rangle>)\<close> and \<open>(\<E>(\<pi> ;; `x \<mapsto> \<langle>e'';\<rho>'';\<kappa>\<rangle>)) \<pi>' = Some (\<langle>e';\<rho>';\<kappa>'\<rangle>)\<close>
-  have "\<parallel>\<rho>'\<parallel> \<sqsubseteq> \<V>" by (blast intro: accept_pool_to_precise)
+  have "\<parallel>\<rho>'\<parallel> \<sqsubseteq> \<V>" by (blast intro: static_eval_pool_to_precise)
 
   assume "\<E> \<pi> = Some (\<langle>LET x = b in e;\<rho>;\<kappa>\<rangle>)"
   with \<open>\<forall>\<pi> e \<rho> \<kappa>. \<E> \<pi> = Some (\<langle>e;\<rho>;\<kappa>\<rangle>) \<longrightarrow> \<V> \<turnstile> e\<^sub>0 \<down> \<pi> \<mapsto> e \<and> \<V> \<tturnstile> e\<^sub>0 \<down> \<pi> \<mapsto> \<kappa>\<close>
@@ -513,13 +513,13 @@ proof -
     assume "b = \<lparr>\<rparr>" and "e'' = e"
     with \<open>\<V> \<turnstile> e\<^sub>0 \<down> \<pi> \<mapsto> LET x = b in e\<close> 
     have "\<V> \<turnstile> e\<^sub>0 \<down> \<pi> \<mapsto> LET x = \<lparr>\<rparr> in e''" by simp then
-    show "\<V> \<turnstile> e\<^sub>0 \<down> \<pi> ;; `x \<mapsto> e''" by (simp add: traceable.Let_Unit)
+    show "\<V> \<turnstile> e\<^sub>0 \<down> \<pi> ;; `x \<mapsto> e''" by (simp add: static_traceable.Let_Unit)
   next
     case (Let_Prim p)
     assume "b = Prim p" and "e'' = e"
     with \<open>\<V> \<turnstile> e\<^sub>0 \<down> \<pi> \<mapsto> LET x = b in e\<close>
     have "\<V> \<turnstile> e\<^sub>0 \<down> \<pi> \<mapsto> LET x = Prim p in e''" by simp then
-    show "\<V> \<turnstile> e\<^sub>0 \<down> \<pi> ;; `x \<mapsto> e''" by (simp add: traceable.Let_Prim)
+    show "\<V> \<turnstile> e\<^sub>0 \<down> \<pi> ;; `x \<mapsto> e''" by (simp add: static_traceable.Let_Prim)
   next
     case (Let_Fst x\<^sub>p x\<^sub>1 x\<^sub>2 \<rho>\<^sub>p \<omega>)
     assume "\<rho>'' = \<rho> ++ [x \<mapsto> \<omega>]"
@@ -528,10 +528,10 @@ proof -
     have "\<V> \<turnstile> e\<^sub>0 \<down> \<pi> \<mapsto> LET x = FST x\<^sub>p in e''" by simp 
     with \<open>(\<V>, \<C>) \<Turnstile>\<^sub>\<E> \<E>(\<pi> ;; `x \<mapsto> \<langle>e'';\<rho>'';\<kappa>\<rangle>)\<close>
     and `\<rho>'' = \<rho> ++ [x \<mapsto> \<omega>]`
-    have "\<parallel>\<rho> ++ [x \<mapsto> \<omega>]\<parallel> \<sqsubseteq> \<V>" using accept_pool_sound by fastforce then
+    have "\<parallel>\<rho> ++ [x \<mapsto> \<omega>]\<parallel> \<sqsubseteq> \<V>" using isnt_static_eval_pool_sound by fastforce then
     have "{|\<omega>|} \<subseteq> \<V> x" using abstracted_value_exists by auto
     with \<open>\<V> \<turnstile> e\<^sub>0 \<down> \<pi> \<mapsto> LET x = FST x\<^sub>p in e''\<close> \<open>{|\<omega>|} \<subseteq> \<V> x\<close> 
-    show "\<V> \<turnstile> e\<^sub>0 \<down> \<pi> ;; `x \<mapsto> e''" by (blast intro: traceable.Let_Fst)
+    show "\<V> \<turnstile> e\<^sub>0 \<down> \<pi> ;; `x \<mapsto> e''" by (blast intro: static_traceable.Let_Fst)
   next
     case (Let_Snd x\<^sub>p x\<^sub>1 x\<^sub>2 \<rho>\<^sub>p \<omega>)
     assume "\<rho>'' = \<rho> ++ [x \<mapsto> \<omega>]"
@@ -540,10 +540,10 @@ proof -
     have "\<V> \<turnstile> e\<^sub>0 \<down> \<pi> \<mapsto> LET x = SND x\<^sub>p in e''" by simp 
     with \<open>(\<V>, \<C>) \<Turnstile>\<^sub>\<E> \<E>(\<pi> ;; `x \<mapsto> \<langle>e'';\<rho>'';\<kappa>\<rangle>)\<close>
     and `\<rho>'' = \<rho> ++ [x \<mapsto> \<omega>]`
-    have "\<parallel>\<rho> ++ [x \<mapsto> \<omega>]\<parallel> \<sqsubseteq> \<V>" using accept_pool_sound by fastforce then
+    have "\<parallel>\<rho> ++ [x \<mapsto> \<omega>]\<parallel> \<sqsubseteq> \<V>" using isnt_static_eval_pool_sound by fastforce then
     have "{|\<omega>|} \<subseteq> \<V> x" using abstracted_value_exists by auto
     with \<open>\<V> \<turnstile> e\<^sub>0 \<down> \<pi> \<mapsto> LET x = SND x\<^sub>p in e''\<close> \<open>{|\<omega>|} \<subseteq> \<V> x\<close> 
-    show "\<V> \<turnstile> e\<^sub>0 \<down> \<pi> ;; `x \<mapsto> e''" by (blast intro: traceable.Let_Snd)
+    show "\<V> \<turnstile> e\<^sub>0 \<down> \<pi> ;; `x \<mapsto> e''" by (blast intro: static_traceable.Let_Snd)
   next
     case (Let_Case_Left x\<^sub>s x\<^sub>l' \<rho>\<^sub>l \<omega>\<^sub>l x\<^sub>l x\<^sub>r e\<^sub>r)
     from `\<kappa> = \<langle>x,e,\<rho>\<rangle> # \<kappa>`
@@ -576,7 +576,7 @@ proof -
 qed
 
 
-lemma traceable_exp_preserved_under_seq_step_up: "
+lemma static_traceable_exp_preserved_under_seq_step_up: "
   \<E> \<rightarrow> \<E>(\<pi> ;; \<upharpoonleft>x \<mapsto> \<langle>e'a;\<rho>'';\<langle>x,e,\<rho>\<rangle> # \<kappa>\<rangle>) \<Longrightarrow>
   (\<E>(\<pi> ;; \<upharpoonleft>x \<mapsto> \<langle>e'a;\<rho>'';\<langle>x,e,\<rho>\<rangle> # \<kappa>\<rangle>)) \<pi>' = Some (\<langle>e';\<rho>';\<kappa>'\<rangle>) \<Longrightarrow>
   \<forall>\<pi> e \<rho> \<kappa>. \<E> \<pi> = Some (\<langle>e;\<rho>;\<kappa>\<rangle>) \<longrightarrow> \<V> \<turnstile> e\<^sub>0 \<down> \<pi> \<mapsto> e \<and> \<V> \<tturnstile> e\<^sub>0 \<down> \<pi> \<mapsto> \<kappa> \<Longrightarrow>
@@ -587,32 +587,32 @@ lemma traceable_exp_preserved_under_seq_step_up: "
 "
   apply (case_tac "\<pi>' = \<pi> ;; \<upharpoonleft>x"; auto)
   apply ((drule spec)+, erule impE, assumption, erule conjE)
-  apply (drule accept_pool_to_precise, auto)
+  apply (drule static_eval_pool_to_precise, auto)
   apply (erule seq_step.cases, auto)
-  apply (drule abstracted_value_exists, simp+, rule traceable.Let_Case_Left; auto)
-  apply (drule abstracted_value_exists, simp+, rule traceable.Let_Case_Right; auto)
-  apply (drule abstracted_value_exists, simp+, rule traceable.Let_App; auto)
+  apply (drule abstracted_value_exists, simp+, rule static_traceable.Let_Case_Left; auto)
+  apply (drule abstracted_value_exists, simp+, rule static_traceable.Let_Case_Right; auto)
+  apply (drule abstracted_value_exists, simp+, rule static_traceable.Let_App; auto)
 done
 
-lemma traceable_exp_preserved_under_chan:"
+lemma static_traceable_exp_preserved_under_chan:"
   (\<E>(\<pi> ;; `x \<mapsto> \<langle>e;\<rho>(x \<mapsto> \<lbrace>Ch \<pi> x\<rbrace>);\<kappa>\<rangle>)) \<pi>' = Some (\<langle>e';\<rho>';\<kappa>'\<rangle>) \<Longrightarrow>
   \<forall>\<pi> e \<rho> \<kappa>. \<E> \<pi> = Some (\<langle>e;\<rho>;\<kappa>\<rangle>) \<longrightarrow> \<V> \<turnstile> e\<^sub>0 \<down> \<pi> \<mapsto> e \<and> \<V> \<tturnstile> e\<^sub>0 \<down> \<pi> \<mapsto> \<kappa> \<Longrightarrow>
   \<E> \<pi> = Some (\<langle>LET x = CHAN \<lparr>\<rparr> in e;\<rho>;\<kappa>\<rangle>) \<Longrightarrow> 
   \<V> \<turnstile> e\<^sub>0 \<down> \<pi>' \<mapsto> e'
 "
-  apply (smt map_upd_Some_unfold state.inject traceable.Let_Chan)
+  apply (smt map_upd_Some_unfold state.inject static_traceable.Let_Chan)
 done
 
-lemma traceable_exp_preserved_under_spawn: "
+lemma static_traceable_exp_preserved_under_spawn: "
   (\<E>(\<pi> ;; `x \<mapsto> \<langle>e;\<rho>(x \<mapsto> \<lbrace>\<rbrace>);\<kappa>\<rangle>, \<pi> ;; .x \<mapsto> \<langle>e\<^sub>c;\<rho>;[]\<rangle>)) \<pi>' = Some (\<langle>e';\<rho>';\<kappa>'\<rangle>) \<Longrightarrow>
   \<forall>\<pi> e \<rho> \<kappa>. \<E> \<pi> = Some (\<langle>e;\<rho>;\<kappa>\<rangle>) \<longrightarrow> \<V> \<turnstile> e\<^sub>0 \<down> \<pi> \<mapsto> e \<and> \<V> \<tturnstile> e\<^sub>0 \<down> \<pi> \<mapsto> \<kappa> \<Longrightarrow>
   \<E> \<pi> = Some (\<langle>LET x = SPAWN e\<^sub>c in e;\<rho>;\<kappa>\<rangle>) \<Longrightarrow> 
   \<V> \<turnstile> e\<^sub>0 \<down> \<pi>' \<mapsto> e'
 "
-  apply (smt map_upd_Some_unfold state.inject traceable.Let_Spawn traceable.Let_Spawn_Child)
+  apply (smt map_upd_Some_unfold state.inject static_traceable.Let_Spawn static_traceable.Let_Spawn_Child)
 done
  
-lemma traceable_exp_preserved_under_sync: "
+lemma static_traceable_exp_preserved_under_sync: "
   \<E> \<rightarrow> \<E>(\<pi>\<^sub>s ;; `x\<^sub>s \<mapsto> \<langle>e\<^sub>s;\<rho>\<^sub>s(x\<^sub>s \<mapsto> \<lbrace>\<rbrace>);\<kappa>\<^sub>s\<rangle>, \<pi>\<^sub>r ;; `x\<^sub>r \<mapsto> \<langle>e\<^sub>r;\<rho>\<^sub>r(x\<^sub>r \<mapsto> \<omega>\<^sub>m);\<kappa>\<^sub>r\<rangle>) \<Longrightarrow>
   (\<E>(\<pi>\<^sub>s ;; `x\<^sub>s \<mapsto> \<langle>e\<^sub>s;\<rho>\<^sub>s(x\<^sub>s \<mapsto> \<lbrace>\<rbrace>);\<kappa>\<^sub>s\<rangle>, \<pi>\<^sub>r ;; `x\<^sub>r \<mapsto> \<langle>e\<^sub>r;\<rho>\<^sub>r(x\<^sub>r \<mapsto> \<omega>\<^sub>m);\<kappa>\<^sub>r\<rangle>)) \<pi>' = Some (\<langle>e';\<rho>';\<kappa>'\<rangle>) \<Longrightarrow>
   \<forall>\<pi> e \<rho> \<kappa>. \<E> \<pi> = Some (\<langle>e;\<rho>;\<kappa>\<rangle>) \<longrightarrow> \<V> \<turnstile> e\<^sub>0 \<down> \<pi> \<mapsto> e \<and> \<V> \<tturnstile> e\<^sub>0 \<down> \<pi> \<mapsto> \<kappa> \<Longrightarrow>
@@ -622,17 +622,17 @@ lemma traceable_exp_preserved_under_sync: "
   \<V> \<turnstile> e\<^sub>0 \<down> \<pi>' \<mapsto> e'
 "
   apply (case_tac "\<pi>' = \<pi>\<^sub>r ;; `x\<^sub>r", auto)
-  apply (drule accept_preserved_under_concur_step, auto)
-  apply (meson traceable_exp_preserved_sync_recv_evt)
+  apply (drule static_eval_preserved_under_concur_step, auto)
+  apply (meson static_traceable_exp_preserved_sync_recv_evt)
   apply (case_tac "\<pi>' = \<pi>\<^sub>s ;; `x\<^sub>s")
-  apply (drule accept_preserved_under_concur_step; auto)
-  apply (meson traceable_exp_preserved_sync_send_evt)
-  apply (smt exp.inject(1) option.inject state.inject traceable_exp_preserved_sync_send_evt)
+  apply (drule static_eval_preserved_under_concur_step; auto)
+  apply (meson static_traceable_exp_preserved_sync_send_evt)
+  apply (smt exp.inject(1) option.inject state.inject static_traceable_exp_preserved_sync_send_evt)
   apply simp
 done
 
 
-lemma traceable_exp_preserved: "
+lemma static_traceable_exp_preserved: "
   \<lbrakk>
     \<E> \<rightarrow> \<E>';
     \<E>' \<pi>' = Some (\<langle>e';\<rho>';\<kappa>'\<rangle>);
@@ -665,7 +665,7 @@ proof -
     and \<open>\<E> \<pi> = Some (\<langle>RESULT x;\<rho>;\<langle>x\<^sub>\<kappa>,e\<^sub>\<kappa>,\<rho>\<^sub>\<kappa>\<rangle> # \<kappa>\<rangle>)\<close>
     and \<open>\<langle>RESULT x;\<rho>;\<langle>x\<^sub>\<kappa>,e\<^sub>\<kappa>,\<rho>\<^sub>\<kappa>\<rangle> # \<kappa>\<rangle> \<hookrightarrow> \<sigma>'\<close>
 
-    show "\<V> \<turnstile> e\<^sub>0 \<down> \<pi>' \<mapsto> e'" by (blast intro: traceable_exp_preserved_under_seq_step_down)
+    show "\<V> \<turnstile> e\<^sub>0 \<down> \<pi>' \<mapsto> e'" by (blast intro: static_traceable_exp_preserved_under_seq_step_down)
   next
     case (Seq_Step \<pi> x b e \<rho> \<kappa>'' e'' \<rho>'')
 
@@ -686,7 +686,7 @@ proof -
     and \<open>\<E> \<pi> = Some (\<langle>LET x = b in e;\<rho>;\<kappa>''\<rangle>)\<close>
     and \<open>\<langle>LET x = b in e;\<rho>;\<kappa>''\<rangle> \<hookrightarrow> \<langle>e'';\<rho>'';\<kappa>''\<rangle>\<close>
 
-    show "\<V> \<turnstile> e\<^sub>0 \<down> \<pi>' \<mapsto> e'" by (auto simp: traceable_exp_preserved_under_seq_step)
+    show "\<V> \<turnstile> e\<^sub>0 \<down> \<pi>' \<mapsto> e'" by (auto simp: static_traceable_exp_preserved_under_seq_step)
   next
     case (Seq_Step_Up \<pi> x b e \<rho> \<kappa> e'' \<rho>'')
 
@@ -708,7 +708,7 @@ proof -
     and \<open>\<E> \<pi> = Some (\<langle>LET x = b in e;\<rho>;\<kappa>\<rangle>)\<close>
     and \<open>\<langle>LET x = b in e;\<rho>;\<kappa>\<rangle> \<hookrightarrow> \<langle>e'';\<rho>'';\<langle>x,e,\<rho>\<rangle> # \<kappa>\<rangle>\<close>
 
-    show "\<V> \<turnstile> e\<^sub>0 \<down> \<pi>' \<mapsto> e'" by (auto simp: traceable_exp_preserved_under_seq_step_up)
+    show "\<V> \<turnstile> e\<^sub>0 \<down> \<pi>' \<mapsto> e'" by (auto simp: static_traceable_exp_preserved_under_seq_step_up)
   next
     case (Let_Chan \<pi> x e \<rho> \<kappa>)
 
@@ -722,7 +722,7 @@ proof -
     with  \<open>\<forall>\<pi> e \<rho> \<kappa>. \<E> \<pi> = Some (\<langle>e;\<rho>;\<kappa>\<rangle>) \<longrightarrow> \<V> \<turnstile> e\<^sub>0 \<down> \<pi> \<mapsto> e \<and> \<V> \<tturnstile> e\<^sub>0 \<down> \<pi> \<mapsto> \<kappa>\<close> 
     and \<open>\<E> \<pi> = Some (\<langle>LET x = CHAN \<lparr>\<rparr> in e;\<rho>;\<kappa>\<rangle>)\<close>
 
-    show "\<V> \<turnstile> e\<^sub>0 \<down> \<pi>' \<mapsto> e'" by (auto simp: traceable_exp_preserved_under_chan)
+    show "\<V> \<turnstile> e\<^sub>0 \<down> \<pi>' \<mapsto> e'" by (auto simp: static_traceable_exp_preserved_under_chan)
   next
     case (Let_Spawn \<pi> x e\<^sub>c e \<rho> \<kappa>)
     assume "\<E>' = \<E> ++ [\<pi> ;; `x \<mapsto> \<langle>e;\<rho> ++ [x \<mapsto> \<lbrace>\<rbrace>];\<kappa>\<rangle>, \<pi> ;; .x \<mapsto> \<langle>e\<^sub>c;\<rho>;[]\<rangle>]"
@@ -734,7 +734,7 @@ proof -
     with \<open>\<forall>\<pi> e \<rho> \<kappa>. \<E> \<pi> = Some (\<langle>e;\<rho>;\<kappa>\<rangle>) \<longrightarrow> \<V> \<turnstile> e\<^sub>0 \<down> \<pi> \<mapsto> e \<and> \<V> \<tturnstile> e\<^sub>0 \<down> \<pi> \<mapsto> \<kappa>\<close> 
     and \<open>\<E> \<pi> = Some (\<langle>LET x = SPAWN e\<^sub>c in e;\<rho>;\<kappa>\<rangle>)\<close>
 
-    show "\<V> \<turnstile> e\<^sub>0 \<down> \<pi>' \<mapsto> e'" by (auto simp: traceable_exp_preserved_under_spawn)
+    show "\<V> \<turnstile> e\<^sub>0 \<down> \<pi>' \<mapsto> e'" by (auto simp: static_traceable_exp_preserved_under_spawn)
   next
     case (Let_Sync \<pi>\<^sub>s x\<^sub>s x\<^sub>s\<^sub>e e\<^sub>s \<rho>\<^sub>s \<kappa>\<^sub>s x\<^sub>s\<^sub>c x\<^sub>m \<rho>\<^sub>s\<^sub>e \<pi>\<^sub>r x\<^sub>r x\<^sub>r\<^sub>e e\<^sub>r \<rho>\<^sub>r \<kappa>\<^sub>r x\<^sub>r\<^sub>c \<rho>\<^sub>r\<^sub>e c \<omega>\<^sub>m)
 
@@ -752,12 +752,12 @@ proof -
     and \<open>\<E> \<pi>\<^sub>s = Some (\<langle>LET x\<^sub>s = SYNC x\<^sub>s\<^sub>e in e\<^sub>s;\<rho>\<^sub>s;\<kappa>\<^sub>s\<rangle>)\<close>
     and \<open>\<E> \<pi>\<^sub>r = Some (\<langle>LET x\<^sub>r = SYNC x\<^sub>r\<^sub>e in e\<^sub>r;\<rho>\<^sub>r;\<kappa>\<^sub>r\<rangle>)\<close>
 
-    show "\<V> \<turnstile> e\<^sub>0 \<down> \<pi>' \<mapsto> e'" by (auto simp: traceable_exp_preserved_under_sync)
+    show "\<V> \<turnstile> e\<^sub>0 \<down> \<pi>' \<mapsto> e'" by (auto simp: static_traceable_exp_preserved_under_sync)
   qed
 qed
 
 
-lemma traceable_stack_preserved: "
+lemma static_traceable_stack_preserved: "
 \<lbrakk>
   \<E> \<rightarrow> \<E>';
   \<E>' \<pi>' = Some (\<langle>e';\<rho>';\<kappa>'\<rangle>);
@@ -771,36 +771,36 @@ apply (frule concur_step.cases, auto)
 apply (case_tac "\<pi>' = \<pi> ;; \<downharpoonleft>x\<^sub>\<kappa>", auto)
 apply ((drule spec)+, erule impE, assumption, erule conjE)
 apply (erule seq_step.cases; auto)
-apply (erule stack_traceable.cases; auto)
-  using Up_Down stack_traceable_preserved_over_balanced_extension apply blast
+apply (erule stack_static_traceable.cases; auto)
+  using Up_Down stack_static_traceable_preserved_over_balanced_extension apply blast
 
 apply (case_tac "\<pi>' = \<pi> ;; `x", auto)
-  using stack_traceable_preserved_over_seq_extension apply blast
+  using stack_static_traceable_preserved_over_seq_extension apply blast
 
 apply (case_tac "\<pi>' = \<pi> ;; \<upharpoonleft>x", auto)
 apply ((drule spec)+, erule impE, assumption, erule conjE) 
-apply (simp add: path_balanced.Empty stack_traceable.Nonempty)
+apply (simp add: path_balanced.Empty stack_static_traceable.Nonempty)
 
 apply (case_tac "\<pi>' = \<pi> ;; `x", auto)
-  using stack_traceable_preserved_over_seq_extension apply blast
+  using stack_static_traceable_preserved_over_seq_extension apply blast
 
 apply (case_tac "\<pi>' = \<pi> ;; .x", auto)
 using Empty_Local path_balanced.Empty apply blast
 apply (case_tac "\<pi>' = \<pi> ;; `x", auto)
-  using stack_traceable_preserved_over_seq_extension apply blast
+  using stack_static_traceable_preserved_over_seq_extension apply blast
 
 
 apply (case_tac "\<pi>' = \<pi>\<^sub>r ;; `x\<^sub>r", auto)
-  apply (simp add: stack_traceable_preserved_over_seq_extension)
+  apply (simp add: stack_static_traceable_preserved_over_seq_extension)
 
 apply (case_tac "\<pi>' = \<pi>\<^sub>s ;; `x\<^sub>s", auto)
-  using stack_traceable_preserved_over_seq_extension apply blast
+  using stack_static_traceable_preserved_over_seq_extension apply blast
 
-  using stack_traceable_preserved_over_seq_extension apply blast
+  using stack_static_traceable_preserved_over_seq_extension apply blast
 
 done
 
-lemma isnt_traceable_sound': "
+lemma isnt_static_traceable_sound': "
   \<lbrakk>
     \<E>\<^sub>0 \<rightarrow>* \<E>
   \<rbrakk> \<Longrightarrow>
@@ -813,19 +813,19 @@ lemma isnt_traceable_sound': "
  apply (drule star_implies_star_left)
  apply (erule star_left.induct; auto)
   apply (simp add: Start)
-  using path_balanced.Empty stack_traceable.Empty apply blast
+  using path_balanced.Empty stack_static_traceable.Empty apply blast
   apply (rename_tac \<E> \<E>' \<pi> e \<rho> \<kappa>)
   apply (drule star_left_implies_star)
-  apply (drule accept_preserved_under_concur_step_star, blast)
-  apply (drule traceable_exp_preserved, auto)
+  apply (drule static_eval_preserved_under_concur_step_star, blast)
+  apply (drule static_traceable_exp_preserved, auto)
  apply (rename_tac \<E> \<E>' \<pi> e \<rho> \<kappa>)
  apply (drule star_left_implies_star)
- apply (drule accept_preserved_under_concur_step_star, blast)
- apply (drule traceable_stack_preserved, auto)
+ apply (drule static_eval_preserved_under_concur_step_star, blast)
+ apply (drule static_traceable_stack_preserved, auto)
 done
 
 
-lemma isnt_traceable_sound: "
+lemma isnt_static_traceable_sound: "
   \<lbrakk>
     (\<V>, \<C>) \<Turnstile>\<^sub>e e\<^sub>0;
     [[] \<mapsto> \<langle>e\<^sub>0;Map.empty;[]\<rangle>] \<rightarrow>* \<E>;
@@ -841,7 +841,7 @@ proof -
   have "(\<V>, \<C>) \<Turnstile>\<^sub>\<E> [[] \<mapsto> \<langle>e\<^sub>0; empty; []\<rangle>]" by (simp add: static_eval_to_pool)
 
   from \<open>(\<V>, \<C>) \<Turnstile>\<^sub>\<E> [[] \<mapsto> \<langle>e\<^sub>0;Map.empty;[]\<rangle>]\<close> \<open>\<E> \<pi> = Some (\<langle>e;\<rho>;\<kappa>\<rangle>)\<close> \<open>[[] \<mapsto> \<langle>e\<^sub>0; empty; []\<rangle>] \<rightarrow>* \<E>\<close>
-  show "\<V> \<turnstile> e\<^sub>0 \<down> \<pi> \<mapsto> e" using isnt_traceable_sound' by blast
+  show "\<V> \<turnstile> e\<^sub>0 \<down> \<pi> \<mapsto> e" using isnt_static_traceable_sound' by blast
 qed
 
   
